theories/TensorAutomation/LtacTensorExprDBParseTemp.v
@@ -1,0 +1,2030 @@
+Require Import Summable.
+Require StringCustomNotation.
+
+From stdpp Require Import strings fin_maps pmap gmap hlist.
+From stdpp Require Import pretty.
+
+Require Import Aux_stdpp.
+Require Import TensorExprDBSyntax.
+
+Require Import Ltac2.Init.
+Require Import LtacTensorExpr.
+Require Import FSetExtra.
+Require UTest.
+
+Require Import ConstrExtra.
+
+
+Ltac2 Type SRData := {
+  ringType : constr;
+  ringO : constr;
+  ringI : constr;
+  ringadd : constr;
+  ringmul : constr;
+  ringeq : constr;
+  ringSR : constr;
+}.
+
+Ltac2 mk_SRData :=
+  fun rT rO rI radd rmul req rSR =>
+  {
+  ringType := rT;
+  ringO := rO;
+  ringI := rI;
+  ringadd := radd;
+  ringmul := rmul;
+  ringeq := req;
+  ringSR := rSR;
+}.
+
+(* Get the SRData for a given type [rT] *)
+Ltac2 get_SRData (rT : constr) :=
+  let rO := (mk_evar rT) in 
+  let rI := (mk_evar rT) in 
+  let radd := (mk_evar '($rT -> $rT -> $rT)) in 
+  let rmul := (mk_evar '($rT -> $rT -> $rT)) in 
+  let req := (mk_evar '($rT -> $rT -> Prop)) in
+  let rSR := (mk_evar '(SemiRing $rT $rO $rI $radd $rmul $req)) in
+  Std.resolve_tc rSR;
+  mk_SRData rT rO rI radd rmul req rSR.
+
+Ltac2 get_summable (tA : constr) :=
+  let sA := mk_evar '(Summable $tA) in 
+  Std.resolve_tc sA;
+  sA.
+
+(*  
+Section test.
+
+Context `{SR : SemiRing R rO rI radd rmul req}.
+
+Import Std.
+Goal true.
+(* Ltac2 Eval Std.unify '(1 : nat) '(2 : nat). *)
+Ltac2 Eval Control.case (fun () => Std.unify '(1 : nat) '(2 : nat)).  false) 
+  (fun _ => false).
+
+Ltac2 Eval Control.plus (fun () => Std.eval_red (* Std.eval_cbn 
+  {
+    Std.rStrength := Std.Norm;
+    Std.rBeta := true;
+    Std.rMatch := true;
+    Std.rFix := true;
+    Std.rCofix := true;
+    Std.rZeta := true;
+    Std.rDelta := true;
+    Std.rConst := [];
+  } *)
+((get_SRData 'R).(ringSR))) (fun _ => 'nat). *)
+
+
+Import Ltac2.Notations.
+
+
+Ltac2 Notation "!if" conds(list1(thunk(tactic(0)), "and")) "then" 
+  t(thunk(tactic(5))) "else" f(thunk(tactic(5))) : 5 :=
+  let rec get_val vs :=
+    match vs with 
+    | [] => false
+    | [v] => v()
+    | v :: vs => 
+      if v() then true else get_val vs
+    end in 
+  if get_val conds then t() else f().
+
+(* Ltac2 Notation "!and" l(thunk(tactic(2))) r(thunk(tactic(2))) : 5 :=
+  if l() then r() else false.
+
+Ltac2 Notation "!or" l(thunk(tactic(2))) r(thunk(tactic(2))) : 5 :=
+  if l() then true else (r()). *)
+
+(* Ltac2 Notation "pattern:" p(pattern) := p. *)
+(* 
+Ltac2 Notation "try" t(thunk(tactic(0))) 
+  "catch" 
+  list1(e(tactic(0)) "default" def(tactic(0)) : 5 :=
+  Control.plus t (fun err => 
+    match err with 
+    | e => def
+    | _ => Control.zero err
+    end). *)
+
+(* Ltac2 Eval 
+  try (Some (Pattern.matches (pattern:(?f ?x ?y)) '(1)) )
+    catch Match_failure default None. *)
+
+
+Ltac2 char_list_of_string (s : string) : char list :=
+  List.map (String.get s) (List.seq 0 1 (String.length s)).
+
+Ltac2 int_of_string (s : string) : int :=
+  List.fold_right (fun c acc => Int.add (Int.sub (Char.to_int c) 48) 
+    (Int.mul 10 acc))
+    (List.rev (char_list_of_string s)) 0.
+
+Ltac2 constr_of_constr_list_typed (type : constr) (l : constr list) : constr :=
+  let rec go l :=
+  match l with 
+  | [] => '(@nil $type)
+  | x :: l' => 
+    let res := go l' in 
+    '(@cons $type $x $res)
+  end in 
+  go l.
+
+Ltac2 constr_of_constr_list (l : constr list) : constr :=
+  let rec go l :=
+  match l with 
+  | [] => 'nil
+  | x :: l' => 
+    let res := go l' in 
+    '(cons $x $res)
+  end in 
+  go l.
+
+Ltac2 constr_of_constr_pair_typed 
+  (ts : constr * constr) : constr * constr -> constr :=
+  fun (a, b) => 
+  let (tA, tB) := ts in 
+  '(@pair $tA $tB $a $b).
+
+Ltac2 constr_of_constr_map (of_k : 'k -> constr) (of_v : 'v -> constr)
+  (tk : constr) (tv : constr) (tm : constr) (m : ('k, 'v) FMap.t) : constr :=
+  let mappings :=
+    constr_of_constr_list_typed '(prod $tk $tv)
+      (List.map (fun (k, v) => 
+        let ck := of_k k with cv := of_v v in 
+        '(@pair $tk $tv $ck $cv)) (FMap.bindings m)) in 
+  let res := '(@list_to_map $tk $tv $tm _ _ $mappings) in 
+  Std.resolve_tc res;
+  res.
+
+Ltac2 constr_of_string (s : string) : constr :=
+  StringCustomNotation.string_name.IdentToString.string_to_coq_string s.
+
+Ltac2 rec constr_of_pos (i : int) : constr :=
+  match Int.compare i 1 with 
+  | 1 => let res := constr_of_pos (Int.asr i 1) in 
+    match Int.land i 1 with
+    | 1 => '(xI $res)
+    | _ => '(xO $res)
+    end
+  | 0 => 'xH
+  | _ =>
+    Control.throw_invalid_argument "constr_of_pos: nonpositive argument"
+  end.
+
+
+Ltac2 rec fold_left' (f : 'a -> 'a -> 'a) (d : 'a) (l : 'a list) : 'a :=
+  let rec go l acc :=
+  match l with 
+  | [] => acc
+  | x :: l => go l (f acc x)
+  end in 
+  match l with 
+  | [] => d
+  | x :: l => go l x
+  end.
+
+Ltac2 rec constr_nat_of_int (i : int) : constr :=
+  if Int.le i 0 then 
+    'O
+  else 
+    let n' := constr_nat_of_int (Int.sub i 1) in 
+    '(S $n').
+
+Ltac2 rec constr_of_tensorexpr (te : TensorExpr) : constr :=
+  match te with 
+  | Abstract name lower upper => 
+    let cname := constr_of_string name in
+    let clower := constr_of_constr_list_typed 'string
+      (List.map (fun (_, s) => constr_of_string s) lower) in 
+    let cupper := constr_of_constr_list_typed 'string
+      (List.map (fun (_, s) => constr_of_string s) upper) in 
+    '(tabstract $cname $clower $cupper)
+  | Product tes => 
+    fold_left' (fun l r => '(tproduct $l $r)) 'tone
+      (List.map constr_of_tensorexpr tes)
+  | Sum (ty, var) smd => 
+    let cty := constr_nat_of_int (int_of_string ty) in 
+    let cvar := constr_of_string var in 
+    let csmd := constr_of_tensorexpr smd in 
+    '(tsum $cvar $cty $csmd)
+  end.
+
+
+Ltac2 rec constr_of_tensorexpr' (te : TensorExpr) : constr :=
+  match te with 
+  | Abstract name lower upper => 
+    let cname := constr_of_string name in
+    let clower := constr_of_constr_list_typed 'string
+      (List.map (fun (_, s) => constr_of_string s) lower) in 
+    let cupper := constr_of_constr_list_typed 'string
+      (List.map (fun (_, s) => constr_of_string s) upper) in 
+    Constr.Unsafe.make (Constr.Unsafe.App '(tabstract) [|cname; clower; cupper|])
+  | Product tes => 
+    fold_left' (fun l r => 
+      Constr.Unsafe.make (Constr.Unsafe.App '(tproduct) [|l; r|])) 'tone
+      (List.map constr_of_tensorexpr' tes)
+  | Sum (ty, var) smd => 
+    let cty := constr_nat_of_int (int_of_string ty) in 
+    let cvar := constr_of_string var in 
+    let csmd := constr_of_tensorexpr' smd in 
+    Constr.Unsafe.make (Constr.Unsafe.App '(tsum) [|cvar; cty; csmd|])
+  end.
+
+(* 
+Ltac2 test_lhs () : TensorExpr :=
+  Product
+  [Sum ("1", "y")
+ (Sum ("0", "x")
+   (Product
+	 [Abstract "f0" [("0", "f")] [("1", "y")]; Abstract 
+      "f" [("0", "x"); ("1", "y")] [("0", "f")]])); Product
+ [Sum ("1", "y")
+  (Sum ("0", "x")
+    (Product
+      [Abstract "f0" [("0", "f")] [("1", "y")]; Abstract 
+       "f" [("0", "x"); ("1", "y")] [("0", "f")]])); Product
+  [Sum ("1", "y")
+   (Sum ("0", "x")
+     (Product
+       [Abstract "f0" [("0", "f")] [("1", "y")]; Abstract 
+        "f" [("0", "x"); ("1", "y")] [("0", "f")]])); Product
+   [Sum ("1", "y")
+    (Sum ("0", "x")
+      (Product
+        [Abstract "f0" [("0", "f")] [("1", "y")]; Abstract 
+         "f" [("0", "x"); ("1", "y")] [("0", "f")]])); Product
+    [Sum ("1", "y")
+     (Sum ("0", "x")
+       (Product
+         [Abstract "f0" [("0", "f")] [("1", "y")]; Abstract 
+          "f" [("0", "x"); ("1", "y")] [("0", "f")]])); Product
+     [Sum ("1", "y")
+      (Sum ("0", "x")
+        (Product
+          [Abstract "f0" [("0", "f")] [("1", "y")]; Abstract 
+           "f" [("0", "x"); ("1", "y")] [("0", "f")]])); Product
+      [Sum ("1", "y")
+       (Sum ("0", "x")
+         (Product
+           [Abstract "f0" [("0", "f")] [("1", "y")]; Abstract 
+            "f" [("0", "x"); ("1", "y")] [("0", "f")]])); Product
+       [Sum ("1", "y")
+        (Sum ("0", "x")
+          (Product
+            [Abstract "f0" [("0", "f")] [("1", "y")]; Abstract 
+             "f" [("0", "x"); ("1", "y")] [("0", "f")]])); Product
+        [Sum ("1", "y")
+         (Sum ("0", "x")
+           (Product
+             [Abstract "f0" [("0", "f")] [("1", "y")]; Abstract 
+              "f" [("0", "x"); ("1", "y")] [("0", "f")]])); Product
+         [Sum ("1", "y")
+          (Sum ("0", "x")
+            (Product
+              [Abstract "f0" [("0", "f")] [("1", "y")]; Abstract 
+               "f" [("0", "x"); ("1", "y")] [("0", "f")]])); Product
+          [Sum ("1", "y")
+           (Sum ("0", "x")
+             (Product
+               [Abstract "f0" [("0", "f")] [("1", "y")]; Abstract 
+                "f" [("0", "x"); ("1", "y")] [("0", "f")]])); Product
+           [Sum ("1", "y")
+            (Sum ("0", "x")
+              (Product
+                [Abstract "f0" [("0", "f")] [("1", "y")]; Abstract 
+                 "f" [("0", "x"); ("1", "y")] [("0", "f")]])); Product
+            [Sum ("1", "y")
+             (Sum ("0", "x")
+               (Product
+                 [Abstract "f0" [("0", "f")] [("1", "y")]; Abstract 
+                  "f" [("0", "x"); ("1", "y")] [("0", "f")]])); Product
+             [Sum ("1", "y")
+              (Sum ("0", "x")
+                (Product
+                  [Abstract "f0" [("0", "f")] [("1", "y")]; Abstract 
+                   "f" [("0", "x"); ("1", "y")] [("0", "f")]])); Product
+              [Sum ("1", "y")
+               (Sum ("0", "x")
+                 (Product
+                   [Abstract "f0" [("0", "f")] [("1", "y")]; Abstract 
+                    "f" [("0", "x"); ("1", "y")] [("0", "f")]])); Product
+               [Sum ("1", "y")
+                (Sum ("0", "x")
+                  (Product
+                    [Abstract "f0" [("0", "f")] [("1", "y")]; Abstract 
+                     "f" [("0", "x"); ("1", "y")] 
+                     [("0", "f")]])); Product
+                [Sum ("1", "y")
+                 (Sum ("0", "x")
+                   (Product
+                     [Abstract "f0" [("0", "f")] [("1", "y")]; Abstract 
+                      "f" [("0", "x"); ("1", "y")] 
+                      [("0", "f")]])); Product
+                 [Sum ("1", "y")
+                  (Sum ("0", "x")
+                    (Product
+                      [Abstract "f0" [("0", "f")] 
+                       [("1", "y")]; Abstract "f" 
+                       [("0", "x"); ("1", "y")] [("0", "f")]])); Product
+                  [Sum ("1", "y")
+                   (Sum ("0", "x")
+                     (Product
+                       [Abstract "f0" [("0", "f")] 
+                        [("1", "y")]; Abstract "f" 
+                        [("0", "x"); ("1", "y")] [("0", "f")]])); Product
+                   [Sum ("1", "y")
+                    (Sum ("0", "x")
+                      (Product
+                        [Abstract "f0" [("0", "f")] 
+                         [("1", "y")]; Abstract "f" 
+                         [("0", "x"); ("1", "y")] 
+                         [("0", "f")]])); Sum ("1", "y")
+                    (Sum ("0", "x")
+                      (Product
+                        [Abstract "f0" [("0", "f")] 
+                         [("1", "y")]; Abstract "f" 
+                         [("0", "x"); ("1", "y")] 
+                         [("0", "f")]]))]]]]]]]]]]]]]]]]]]]].
+
+Ltac2 test_rhs () : TensorExpr := Product
+  [Sum ("1", "y")
+ (Sum ("0", "x")
+   (Product
+	 [Abstract "f0" [("0", "f")] [("1", "y")]; Abstract 
+      "f" [("0", "x"); ("1", "y")] [("0", "f")]])); Product
+ [Sum ("1", "y")
+  (Sum ("0", "x")
+    (Product
+      [Abstract "f0" [("0", "f")] [("1", "y")]; Abstract 
+       "f" [("0", "x"); ("1", "y")] [("0", "f")]])); Product
+  [Sum ("1", "y")
+   (Sum ("0", "x")
+     (Product
+       [Abstract "f0" [("0", "f")] [("1", "y")]; Abstract 
+        "f" [("0", "x"); ("1", "y")] [("0", "f")]])); Product
+   [Sum ("1", "y")
+    (Sum ("0", "x")
+      (Product
+        [Abstract "f0" [("0", "f")] [("1", "y")]; Abstract 
+         "f" [("0", "x"); ("1", "y")] [("0", "f")]])); Product
+    [Sum ("1", "y")
+     (Sum ("0", "x")
+       (Product
+         [Abstract "f0" [("0", "f")] [("1", "y")]; Abstract 
+          "f" [("0", "x"); ("1", "y")] [("0", "f")]])); Product
+     [Sum ("1", "y")
+      (Sum ("0", "x")
+        (Product
+          [Abstract "f0" [("0", "f")] [("1", "y")]; Abstract 
+           "f" [("0", "x"); ("1", "y")] [("0", "f")]])); Sum 
+      ("1", "y")
+      (Sum ("0", "x")
+        (Product
+          [Abstract "f0" [("0", "f")] [("1", "y")]; Abstract 
+           "f" [("0", "x"); ("1", "y")] [("0", "f")]]))]]]]]].
+
+Time Ltac2 Eval 
+  let _ := constr_of_tensorexpr (test_lhs()) in ().
+Time Ltac2 Eval 
+  let _ := constr_of_tensorexpr' (test_lhs()) in (). *)
+
+Ltac2 mutable check_summable := false.
+
+Ltac2 Type Var := [
+  | Rel (int)
+  | Loc (int)
+  | Glob (int)
+].
+
+Ltac2 Type AbsIdx := int.
+Ltac2 abs_tag : AbsIdx FSet.Tags.tag := FSet.Tags.int_tag.
+Ltac2 Type VarIdx := int.
+Ltac2 var_tag : VarIdx FSet.Tags.tag := FSet.Tags.int_tag.
+Ltac2 Type AbsData := AbsIdx * Var list * Var list.
+
+Ltac2 Type TEContext := {
+  ctx_SR : SRData;
+  ctx_vs : (constr * constr) list;
+  ctx_abs : (AbsIdx, constr * int list * int list) FMap.t;
+  ctx_mg : (VarIdx, int * constr) FMap.t;
+  ctx_ml : int list; (* The types of the local variables 
+    [Rel (length ctx_mr + i)], given by indices in ctx_vs *)
+  ctx_mr : int list (* The types of the relative variables, given by 
+    indices in ctx_vs *)
+}.
+
+Ltac2 mk_TEContext (ctx_SR : SRData)
+  (ctx_vs : (constr * constr) list)
+  (ctx_abs : (AbsIdx, constr * int list * int list) FMap.t)
+  (ctx_mg : (VarIdx, int * constr) FMap.t) ctx_ml ctx_mr : TEContext := {
+  ctx_SR := ctx_SR;
+  ctx_vs := ctx_vs;
+  ctx_abs := ctx_abs;
+  ctx_mg := ctx_mg;
+  ctx_ml := ctx_ml;
+  ctx_mr := ctx_mr;
+}.
+
+Ltac2 empty_TEContext (cR : constr) : TEContext :=
+  mk_TEContext (get_SRData cR) 
+    [] (FMap.empty abs_tag) (FMap.empty var_tag)
+    [] [].
+
+Ltac2 fresh_idx (used : int FSet.t) : int :=
+  let rec go n :=
+    if FSet.mem n used then 
+      go (Int.add 1 n)
+    else n
+    in
+  go 1.
+
+
+Ltac2 fresh_idx_of_list (used : int list) : int :=
+  fresh_idx (FSet.of_list FSet.Tags.int_tag used).
+
+
+Ltac2 fresh_idx_of_map (used : (int, 'a) FMap.t) : int :=
+  fresh_idx (FMap.domain used).
+
+Ltac2 fresh_string (used : string FSet.t) (base : string) : string :=
+  (* let base := Option.default "" base in  *)
+  let rec go n := 
+    let s := String.app base (string_of_int n) in 
+    if FSet.mem s used then 
+      go (Int.add n 1)
+    else
+      s
+  in
+  go 0.
+
+Ltac2 fresh_string_of_list (s : string list) (base : string) : string :=
+  fresh_string (FSet.of_list string_tag s) base.
+
+Ltac2 fresh_string_of_map (m : (string, 'a) FMap.t) (base : string) : string :=
+  fresh_string (FMap.domain m) base.
+
+(* Find a type in the [vs] map, adding it if necessary *)
+Ltac2 lookup_vs (vs : (constr * constr) list) (tA : constr) (sA : constr) : 
+  (constr * constr) list * int :=
+  let rec go i vs' :=
+  match vs' with 
+  | [] => (List.append vs [(tA, sA)], i)
+  | (tB, sB) :: vs'' => 
+    !if (unify_eq tA tB) and check_summable and (unify_eq sA sB) then
+      (vs, i)
+    else 
+      go (Int.add i 1) vs''
+  end in 
+  go 0 vs.
+
+(* Find a type in the [vs] map, adding it if necessary *)
+Ltac2 lookup_vs_no_sum (vs : (constr * constr) list) (tA : constr) : 
+  (constr * constr) list * int :=
+  let rec go i vs' :=
+  match vs' with 
+  | [] => 
+    let sA := get_summable tA in 
+    (List.append vs [(tA, sA)], i)
+  | (tB, _sB) :: vs'' => 
+    if (unify_eq tA tB) then
+      (vs, i)
+    else 
+      go (Int.add i 1) vs''
+  end in 
+  go 0 vs.
+
+Ltac2 ctx_lookup_type (ctx : TEContext) (tA : constr) (sA : constr) : 
+  TEContext * int :=
+  let (vs, ty) := lookup_vs (ctx.(ctx_vs)) tA sA in 
+  ({ctx with ctx_vs := vs}, ty).
+
+Ltac2 ctx_lookup_type_no_sum (ctx : TEContext) (tA : constr) : 
+  TEContext * int :=
+  let (vs, ty) := lookup_vs_no_sum (ctx.(ctx_vs)) tA in 
+  ({ctx with ctx_vs := vs}, ty).
+
+(* FIXME: Move *)
+Ltac2 pair_equal (eqa : 'a -> 'a -> bool) (eqb : 'b -> 'b -> bool) : 
+  'a * 'b -> 'a * 'b -> bool :=
+  fun (a, b) (a', b') => if eqa a a' then eqb b b' else false.
+
+Ltac2 parse_var (vs : (constr * constr) list) 
+  (mg : (VarIdx, int * constr) FMap.t)
+  (numrel : int) (* The number of binding local summands *)
+  (val : constr) (type : constr) : 
+  (constr * constr) list * (VarIdx, int * constr) FMap.t * (int * Var) :=
+  let (vs, ty) := lookup_vs_no_sum vs type in 
+  match Unsafe.is_Rel_data val with 
+  | Some i => 
+    if Int.le i numrel then (* le because everything is 1-indexed *)
+      (vs, mg, (ty, Rel i))
+    else (* Local variable *)
+      (vs, mg, (ty, Loc (Int.sub i numrel)))
+  | None =>
+    (* TODO: Replace unify_eq with Unification.conv_full, in Rocq 9.0 *)
+    match FMap.find_inv_opt (pair_equal Int.equal unify_eq) (ty, val) mg with 
+    | Some idx => (vs, mg, (ty, Glob idx))
+    | None => let name := fresh_idx_of_map mg in 
+      (vs, FMap.add name (ty, val) mg, (ty, Glob name))
+    end
+  end.
+
+Ltac2 parse_abs_val 
+  (abs : (AbsIdx, constr * int list * int list) FMap.t)
+  (f : constr) (low : int list) (up : int list) : 
+  (AbsIdx, constr * int list * int list) FMap.t * AbsIdx :=
+  let get_eq (f, low, up) (f', low', up') :=
+    !if (unify_eq f f') and (List.equal Int.equal low low') and 
+      (List.equal Int.equal up up') then true else false in 
+  match FMap.find_inv_opt get_eq (f, low, up) abs with 
+  | Some idx => (abs, idx)
+  | None => let name := fresh_idx_of_map abs in 
+    (FMap.add name (f, low, up) abs, name)
+  end.
+
+Ltac2 parse_abs_data (vs : (constr * constr) list) 
+  (abs : (AbsIdx, constr * int list * int list) FMap.t) 
+  (mg : (VarIdx, int * constr) FMap.t) (numrel : int)
+  (head : constr) (lower : (constr * constr) list)
+  (upper : (constr * constr) list) :
+  (constr * constr) list * (AbsIdx, constr * int list * int list) FMap.t * 
+  (VarIdx, int * constr) FMap.t *
+  AbsData :=
+  let (vs, mg, lower_tyvars) :=
+    List.fold_right (fun (val, type) (vs, vars, tyvars) => 
+      let (vs, vars, tyvar) := parse_var vs vars numrel val type in 
+      (vs, vars, tyvar :: tyvars)) lower (vs, mg, []) in 
+  let (vs, mg, upper_tyvars) :=
+    List.fold_right (fun (val, type) (vs, vars, tyvars) => 
+      let (vs, vars, tyvar) := parse_var vs vars numrel val type in 
+      (vs, vars, tyvar :: tyvars)) upper (vs, mg, []) in 
+  let (abs, abs_idx) := parse_abs_val abs head 
+    (List.map fst lower_tyvars) (List.map fst upper_tyvars) in 
+  (vs, abs, mg, (abs_idx, List.map snd lower_tyvars, List.map snd upper_tyvars)).
+
+
+Ltac2 ctx_parse_var ctx val type :=
+  let (vs, vars, tyvar) := 
+    parse_var (ctx.(ctx_vs)) (ctx.(ctx_mg)) (List.length (ctx.(ctx_mr))) val type in  
+  ({ctx with ctx_vs := vs; ctx_mg := vars}, tyvar).
+
+Ltac2 ctx_parse_abs_val ctx f low up :=
+  let (abs, idx) := parse_abs_val (ctx.(ctx_abs)) f low up in  
+  ({ctx with ctx_abs := abs}, idx).
+
+Ltac2 ctx_parse_abs_data ctx head lower upper :=
+  let (vs, abs, mg, absdata) :=
+    parse_abs_data (ctx.(ctx_vs)) (ctx.(ctx_abs)) (ctx.(ctx_mg))
+      (List.length (ctx.(ctx_mr)))
+      head lower upper in 
+  ({ctx with ctx_vs := vs; ctx_mg := mg; ctx_abs := abs}, 
+    absdata).
+
+
+Import PrintingExtra Pp.
+
+Ltac2 helper_make_typing_map (vs : (constr * constr) list)
+  (ml : int list) (mr : int list) : (int, constr) FMap.t :=
+  FMap.of_list FSet.Tags.int_tag (
+    List.mapi (fun i ty => (Int.add 1 i, fst (List.nth vs ty)))
+    (List.rev (List.append ml mr))).
+
+
+Ltac2 Type rec TensorExprDB := [
+  TOne
+| Abstract (AbsIdx, Var list, Var list) 
+    (* An abstract tensor, along with the registers to which it is 
+      applied as inputs and as outputs, respectively.
+      Each index is stored along with its type. *)
+| Product (TensorExprDB, TensorExprDB)
+    (* The product of a list of tensor expressions, 
+      conventionally left-associated *)
+| Sum (int, TensorExprDB) 
+    (* The sum/contraction of a tensor expression with respect to a
+      given variable *)
+].
+
+Ltac2 rec parse_tensor_expr_aux_data
+  (r : SRData)
+  (to_abs : constr -> (* the constr to decompose. Note it will likely be unsafe 
+    by containing [Rel _] terms. All these will be mapped in [relmap], however *)
+    (int, constr) FMap.t -> (* The typing map for [Rel _] derived from 
+      [relmap] and [vs] (i.e. [Rel i] has type [T = nth vs j] where [relmap !! i = (j, _)]) *)
+    (constr * (* head symbol *)
+      (constr * constr) list * (* lower arguments and their types *)
+      (constr * constr) list (* upper arguments and their types *)) option) 
+  (vs : (constr * constr) list) 
+  (abs : (AbsIdx, constr * int list * int list) FMap.t) 
+  (mg : (VarIdx, int * constr) FMap.t) (ml : int list) (mr : int list)
+  (c : constr) : 
+  (constr * constr) list * (AbsIdx, constr * int list * int list) FMap.t * 
+    (VarIdx, int * constr) FMap.t * int list * int list * TensorExprDB :=
+  let rec go vs abs mg ml mr c : 
+    (constr * constr) list * (AbsIdx, constr * int list * int list) FMap.t * 
+      (VarIdx, int * constr) FMap.t * int list * int list * TensorExprDB :=
+  (* let rT := r.(ringType) in  *)
+  (* print (str "go" ++ spc() ++ of_list (of_pair of_constr of_constr) vs ++
+    spc() ++ print_map of_string of_constr abs ++ 
+    spc() ++ print_map of_string of_constr vars ++
+    spc() ++ of_list (of_pair of_int of_string) rels ++
+    spc() ++ of_constr c);
+  print (mt()); *)
+  if unify_eq c (r.(ringI)) then (vs, abs, mg, ml, mr, TOne) else
+  match! c with 
+  | @sum_of _  _ _  _ _  _  _  ?tA ?sA ?f =>
+      let (vs', idx_A) := lookup_vs vs tA sA in 
+      let (_b, fbody) := Unsafe.decompose_lambda f in 
+      let mr := idx_A :: mr in
+      let (vs, abs, mg, ml, mr, body_te) :=
+        go vs' abs mg ml mr
+          fbody in
+      (vs, abs, mg, ml, List.tl mr, Sum idx_A body_te)
+      (* Product [] *)
+      (* let rels := () *)
+  | ?mul ?a ?b => 
+    Std.unify mul (r.(ringmul));
+    (* print (str "vs: " ++ of_list (of_pair of_constr of_constr) vs); *)
+    let (vs, abs, mg, ml, mr, tea) := 
+      go vs abs mg ml mr a in 
+    (* print (str "vs': " ++ of_list (of_pair of_constr of_constr) vs'); *)
+    let (vs, abs, mg, ml, mr, teb) :=
+      go vs abs mg ml mr b in
+    (* print (str "vs'': " ++ of_list (of_pair of_constr of_constr) vs''); *)
+    (vs, abs, mg, ml, mr, Product tea teb)
+  (* | _ => None *)
+  | _ => 
+    (* print (str "rel_typing_map for " ++ of_constr c ++ str " from: " ++ 
+      of_list (of_pair of_int of_string) rels ++ spc() ++
+      str "vs: " ++ of_list (of_pair of_constr of_constr) vs); *)
+    let rel_typing_map := helper_make_typing_map vs ml mr in 
+    match to_abs c rel_typing_map with 
+    | None => Control.throw (Invalid_argument (Some (
+      Message.concat (Message.of_string "Could not parse constr as TensorExpr: ")
+        (Message.of_constr c)))) 
+    | Some (head, lower, upper) => 
+    (* print (str "_vs: " ++ of_list (of_pair of_constr of_constr) vs); *)
+      let (vs, abs, mg, (idx, l, u)) := 
+        parse_abs_data vs abs mg (List.length mr) head lower upper in 
+    (* print (str "_vs': " ++ of_list (of_pair of_constr of_constr) vs'); *)
+      (vs, abs, mg, ml, mr, Abstract idx l u)
+    end
+  end in 
+  go vs abs mg ml mr c. 
+
+
+
+(** The function which parses abstract values (until extended, always fails!). 
+  To extend this to other functions, do something like the following:
+  Ltac2 Set parse_abstract as parse_abstract_old := fun c relmap => 
+    lazy_match! c with
+    | f ?x ?y ?z => Some ('f, [(x, 'A); (y, 'B)], [(z, 'A)])
+    | _ => parse_abstract_old c relmap
+    end. *)
+Ltac2 mutable parse_abstract : constr -> (* the constr to decompose. Note it will likely be unsafe 
+    by containing [Rel _] terms. All these will be mapped in [relmap], however *)
+    (int, constr) FMap.t -> (* The typing map for [Rel _] derived from 
+      [relmap] and [vs] (i.e. [Rel i] has type [T = nth vs j] where [relmap !! i = (j, _)]) *)
+    (constr * (* head symbol *)
+      (constr * constr) list * (* lower arguments and their types *)
+      (constr * constr) list (* upper arguments and their types *)) option :=
+  fun _c _relmap =>
+  None.
+
+Ltac2 parse_tensor_expr_aux 
+  (ctx : TEContext) (c : constr) : 
+  TEContext * TensorExprDB :=
+  let (vs, abs, mg, ml, mr, te) := 
+    parse_tensor_expr_aux_data (ctx.(ctx_SR)) parse_abstract 
+      (ctx.(ctx_vs)) (ctx.(ctx_abs)) 
+      (ctx.(ctx_mg)) (ctx.(ctx_ml)) (ctx.(ctx_mr)) c in 
+  ({ctx with ctx_vs := vs; ctx_abs := abs; ctx_mg := mg; 
+    ctx_ml := ml; ctx_mr := mr}, te).
+
+
+Ltac2 parse_tensor_equality_aux ctx c : 
+  TEContext * TensorExprDB * TensorExprDB :=
+  let rec go ctx c : 
+    TEContext * TensorExprDB * TensorExprDB :=
+  (* let rT := r.(ringType) in  *)
+  (* print (str "go" ++ spc() ++ of_list (of_pair of_constr of_constr) vs ++
+    spc() ++ print_map of_string of_constr abs ++ 
+    spc() ++ print_map of_string of_constr vars ++
+    spc() ++ of_list (of_pair of_int of_string) rels ++
+    spc() ++ of_constr c);
+  print (mt()); *)
+  match! c with 
+  | ?req ?lhs ?rhs => 
+    Std.unify req (ctx.(ctx_SR).(ringeq));
+    let (ctx, telhs) := parse_tensor_expr_aux ctx lhs in 
+    let (ctx, terhs) := parse_tensor_expr_aux ctx rhs in 
+    (ctx, telhs, terhs)
+  | _ => 
+    let (b, cbody) := Unsafe.decompose_prod c in 
+    let tA := Constr.Binder.type b in 
+    let (ctx, idx_A) := ctx_lookup_type_no_sum ctx tA in 
+    let ml := idx_A :: ctx.(ctx_ml) in
+    go ({ctx with ctx_ml := ml}) cbody
+  end in 
+  go ctx c.
+
+
+(* TODO: Helper function for parsing vector terms into split lists
+Ltac2  *)
+
+
+
+
+
+
+Require Import TensorExprDBSemantics.
+
+Definition unit_Summable@{u} : Summable (unit : Type@{u}) :=
+  (@sum_over (unit : Type@{u}) [ () ]).
+
+Notation SummableType := ({A : Type & Summable A}).
+
+Definition Summable_Type_inhabited : 
+  Inhabited SummableType :=
+  populate (existT (unit : Type) unit_Summable).
+
+Ltac2 get_cV (vs : (constr * constr) list) : constr :=
+  let cVs := constr_of_constr_list_typed 'SummableType
+    (List.map (fun (tA, sA) => '(@existT _ Summable $tA $sA)) vs) in 
+  '(fun (i : Ty) => 
+    projT1 (@lookup_total Ty SummableType (list SummableType)
+    (@list_lookup_total _ Summable_Type_inhabited) i $cVs)).
+
+
+Ltac2 get_cVsum (vs : (constr * constr) list) : constr :=
+  let cVs := constr_of_constr_list_typed 'SummableType
+    (List.map (fun (tA, sA) => '(@existT _ Summable $tA $sA)) vs) in 
+  '(fun (i : Ty) => 
+    projT2 (@lookup_total Ty SummableType (list SummableType)
+    (@list_lookup_total _ Summable_Type_inhabited) i $cVs)).
+
+
+Ltac2 constr_of_typed_fun (cR : constr) (cV : constr (* : Ty -> Type *)) : 
+  constr * int list * int list -> constr :=
+  fun (f, low, up) => 
+  let args := constr_of_constr_list_typed 'nat
+    (List.map constr_nat_of_int (List.append low up)) in 
+  '(@mk_Vfunc $cR $cV $args $f).
+
+Ltac2 constr_of_typed_var (cV : constr) : 
+  int * constr -> constr :=
+  fun (ty, val) => 
+  let cty := constr_nat_of_int ty in 
+  '(@mk_Vval $cV $cty $val).
+
+(* Ltac2 Eval constr_of_constr_map 
+  StringCustomNotation.string_name.IdentToString.string_to_coq_string
+  (fun x => x)
+  'string 'nat '(gmap string N)
+  (FMap.of_list string_tag [("a", '1); ("b", '1)]). *)
+
+Ltac2 constr_of_var (v : Var) : constr :=
+  match v with 
+  | Rel r => let i := constr_of_pos r in 
+    '(rel $i)
+  | Loc l => let i := constr_of_pos l in 
+    '(loc $i)
+  | Glob g => let i := constr_of_pos g in 
+    '(glob $i)
+  end.
+
+Ltac2 rec constr_of_tensorexprdb (te : TensorExprDB) : constr :=
+  match te with
+  | TOne => 'tone
+  | Abstract f low up =>
+    let cf := constr_of_pos f with
+     clow := constr_of_constr_list_typed 'var (List.map constr_of_var low) with
+     cup := constr_of_constr_list_typed 'var (List.map constr_of_var up) in 
+    '(tabstract $cf $clow $cup)
+  | Product l r => 
+    let cl := constr_of_tensorexprdb l in 
+    let cr := constr_of_tensorexprdb r in 
+    '(tproduct $cl $cr)
+  | Sum ty body =>
+    let cty := constr_nat_of_int ty in 
+    let cbody := constr_of_tensorexprdb body in 
+    '(tsum $cty $cbody)
+  end.
+
+Ltac2 ctx_get_cV (ctx : TEContext) : constr :=
+  get_cV (ctx.(ctx_vs)).
+
+Ltac2 ctx_get_cVsum (ctx : TEContext) : constr :=
+  get_cVsum (ctx.(ctx_vs)).
+
+Ltac2 ctx_get_cR (ctx : TEContext) : constr :=
+  ctx.(ctx_SR).(ringType).
+
+Ltac2 ctx_get_cabs (ctx : TEContext) : constr :=
+  let cV := ctx_get_cV ctx in 
+  let cR := ctx_get_cR ctx in 
+  constr_of_constr_map constr_of_pos 
+    (constr_of_typed_fun cR cV) 
+    'positive '(@Vfunc $cR $cV) '(Pmap (@Vfunc $cR $cV)) (ctx.(ctx_abs)).
+
+Ltac2 ctx_get_cmg (ctx : TEContext) : constr :=
+  let cV := ctx_get_cV ctx in 
+  constr_of_constr_map constr_of_pos (constr_of_typed_var cV)
+    'positive '(Vval $cV) '(Pmap (Vval $cV)) (ctx.(ctx_mg)).
+
+Ltac2 ctx_get_ml_list (ctx : TEContext) : (int * int) list :=
+  (List.mapi (fun idx ty => (Int.add 1 idx, ty)) (List.rev (ctx.(ctx_ml)))).
+
+Ltac2 ctx_get_ml_map (ctx : TEContext) : (int, int) FMap.t :=
+  FMap.of_list FSet.Tags.int_tag 
+    (ctx_get_ml_list ctx).
+
+Ltac2 ctx_get_cml (ctx : TEContext) : constr :=
+  constr_of_constr_map constr_of_pos constr_of_pos
+    'positive 'positive '(Pmap positive) (ctx_get_ml_map ctx).
+
+Ltac2 constr_of_pair_typed (ts : constr * constr) 
+  (cA : 'a -> constr) (cB : 'b -> constr) : 'a * 'b -> constr :=
+  fun (a, b) => constr_of_constr_pair_typed ts (cA a, cB b).
+
+Ltac2 ctx_get_cml_list (ctx : TEContext) : constr (*list (Idx * Ty) *):=
+  constr_of_constr_list_typed '(prod Idx Ty) 
+    (List.rev_map (constr_of_pair_typed ('Idx, 'Ty) constr_of_pos constr_nat_of_int)
+      (ctx_get_ml_list ctx)). 
+
+
+
+Ltac2 constr_semantics_of_tensorexpr_aux (ctx : TEContext) (cte : constr) :=
+  let cSR := ctx.(ctx_SR).(ringSR) in 
+  let cV := ctx_get_cV ctx in 
+  let cVsum := ctx_get_cVsum ctx in 
+  let cabs := ctx_get_cabs ctx in 
+  let cmg := ctx_get_cmg ctx in 
+  (* let cml := ctx_get_cml ctx in  *)
+  '(@total_semantics_aux _ _ _ _ _ _ $cSR $cV $cVsum $cabs $cmg ∅ [] $cte).
+
+Ltac2 constr_semantics_of_tensorexpr (ctx : TEContext) (te : TensorExprDB) :=
+  constr_semantics_of_tensorexpr_aux ctx (constr_of_tensorexprdb te).
+
+
+Ltac2 constr_semantics_of_tensor_equality (ctx : TEContext) 
+  (lhs : TensorExprDB) (rhs : TensorExprDB) :=
+  let cSR := ctx.(ctx_SR).(ringSR) in 
+  let cV := ctx_get_cV ctx in 
+  let cVsum := ctx_get_cVsum ctx in 
+  let cabs := ctx_get_cabs ctx in 
+  let cmg := ctx_get_cmg ctx in 
+  let cml := ctx_get_cml_list ctx in 
+  let clhs := constr_of_tensorexprdb lhs in 
+  let crhs := constr_of_tensorexprdb rhs in 
+  (* let cml := ctx_get_cml ctx in  *)
+  '(@tensorequation_semantics_aux _ _ _ _ _ _ $cSR $cV $cVsum $cabs $cmg [] 
+    $clhs $crhs $cml (@empty _ Pmap_empty)).
+
+
+Ltac2 test_parse_tensor_equality (cR : constr) (tH : constr) : unit :=
+  let ctx := empty_TEContext cR in 
+  let (eqctx, lhs, rhs) := parse_tensor_equality_aux ctx tH in 
+  let sem := constr_semantics_of_tensor_equality eqctx lhs rhs in 
+  assert ($tH = $sem).
+  
+Ltac2 test_parse_tensorexpr (c : constr) : unit :=
+  let cR := Constr.type c in 
+  let ctx := empty_TEContext cR in 
+  let (ctx, te) := parse_tensor_expr_aux ctx c in 
+  let sem := constr_semantics_of_tensorexpr ctx te in
+  assert ($c = $sem).
+
+
+Ltac2 pos_of_constr (p : constr) : int :=
+  let rec go p :=
+  match! p with 
+  | xH => 1
+  | xI ?p => Int.add 1 (Int.lsl (go p) 1)
+  | xO ?p => Int.lsl (go p) 1
+  | _ =>
+    let p' := Std.eval_red p in 
+    if Constr.equal p' p then 
+      let p' := Std.eval_vm None p in 
+      if Constr.equal p' p then 
+        Control.throw_invalid_argument 
+          "pos_of_constr: argument is not reducible to a [positive] constant"
+      else go p'
+    else go p'
+  end in 
+  go p.
+
+(* TODO: Support big numbers (Nat.of_num_uint, etc.)*)
+Ltac2 nat_of_constr (n : constr) : int :=
+  let rec go p :=
+  match! p with 
+  | O => 0
+  | S ?n => Int.add 1 (go n)
+  | _ =>
+    let n' := Std.eval_red n in 
+    if Constr.equal n' n then 
+      let n' := Std.eval_vm None n in 
+      if Constr.equal n' n then 
+      Control.throw_invalid_argument 
+        "nat_of_constr: argument is not reducible to a [nat] constant"
+      else go n'
+    else go n'
+  end in 
+  go n.
+
+
+Ltac2 list_of_constr (f : constr -> 'a) : constr -> 'a list :=
+  let rec go l :=
+  match! l with 
+  | nil => []
+  | ?x :: ?l => f x :: go l
+  | _ =>
+    let l' := Std.eval_red l in 
+    if Constr.equal l' l then 
+      Control.throw_invalid_argument 
+        "nat_of_constr: argument is not reducible to a [nat] constant"
+    else go l'
+  end in 
+  go.
+
+Ltac2 var_of_constr (v : constr) : Var :=
+  let rec go v :=
+  match! v with 
+  | rel ?r => Rel (pos_of_constr r)
+  | loc ?l => Loc (pos_of_constr l)
+  | glob ?g => Glob (pos_of_constr g)
+  | _ => 
+    let v' := Std.eval_red v in 
+    if Constr.equal v' v then 
+      let v' := Std.eval_vm None v in 
+      if Constr.equal v' v then 
+      Control.throw_invalid_argument 
+        "nat_of_constr: argument is not reducible to a [nat] constant"
+      else go v'
+    else go v'
+  end in 
+  go v.
+
+Ltac2 tensorexprdb_of_constr (cte : constr) : TensorExprDB :=
+  let rec go cte :=
+  match! cte with
+  | tone => TOne
+  | tabstract ?f ?low ?up => 
+    let vars_of_constr := list_of_constr var_of_constr in 
+    Abstract (pos_of_constr f) (vars_of_constr low) (vars_of_constr up)
+  | tproduct ?l ?r => 
+    Product (go l) (go r)
+  | tsum ?ty ?body => 
+    Sum (nat_of_constr ty) (go body)
+  end in 
+  go cte.
+
+(* Overwrite this to add simplification after rewriting *)
+Ltac2 mutable red_te_semantics_post () : unit :=
+  ().
+
+Ltac2 red_te_semantics () : unit := 
+  lazy [
+  lookup_total list_lookup_total 
+  insert map_insert 
+  partial_alter Pmap_partial_alter 
+    pmap.Pmap_partial_alter_aux pmap.Pmap_ne_partial_alter
+    pmap.Pmap_ne_case pmap.PNode pmap.Pmap_ne_singleton
+  empty Pmap_empty
+
+  list_to_map fold_right
+
+  projT1 fst snd
+
+  tensorequation_semantics_aux
+  total_semantics_aux 
+
+  abstract_semantics 
+  join_list from_option id
+  app
+  mbind option_bind
+  fmap list_fmap option_fmap option_map
+
+  get_var
+  
+  lookup Pmap_lookup Pmap_ne_lookup
+  list_lookup pos_to_nat_pred 
+  Nat.pred Pos.to_nat Pos.iter_op Nat.add
+  
+  Vapplys Vapply Vconst Vval_get
+  mk_Vfunc mk_Vval
+
+  decide decide_rel Nat.eq_dec PeanoNat.Nat.eq_dec
+    nat_rec nat_rect f_equal_nat f_equal eq_rect_r eq_sym eq_rect
+  ];
+  red_te_semantics_post ().
+
+Ltac2 te_rewrite_in_lhs (cR : constr) (tH : constr) : unit :=
+  let goalctx := empty_TEContext cR in 
+  let (goalctx, glhs, grhs) := parse_tensor_equality_aux goalctx (Control.goal()) in 
+  let hypctx := {goalctx with ctx_ml := [] } in 
+  let (hypctx, hlhs, hrhs) := parse_tensor_equality_aux hypctx tH in 
+  let goalml := goalctx.(ctx_ml) in 
+  let ctx := {hypctx with ctx_ml := goalml} in 
+
+  let cglhs := constr_of_tensorexprdb glhs in 
+  let chlhs := constr_of_tensorexprdb hlhs in 
+  let chrhs := constr_of_tensorexprdb hrhs in 
+  let rew_expr := '(match_rewrite_tensorlist (tensorlist_of_tensorexpr $chlhs) 
+    (tensorlist_of_tensorexpr $chrhs) (tensorlist_of_tensorexpr $cglhs)) in 
+  let new_lhs_expr := Std.eval_vm None rew_expr in 
+  lazy_match! new_lhs_expr with 
+  | None => Control.zero (Tactic_failure
+    (Some (Message.of_string "te_rewrite_in_lhs: no rewrite found!")))
+  | Some ?e => 
+    let new_lhs_expr := '(tensorexpr_of_tensorlist $e) in 
+    let new_lhs_expr := Std.eval_vm None new_lhs_expr in
+    let new_lhs := tensorexprdb_of_constr new_lhs_expr in 
+    let new_goal := constr_semantics_of_tensor_equality ctx new_lhs grhs in 
+    enough ($new_goal) by Control.shelve();
+    red_te_semantics()
+  end.
+
+
+Ltac2 te_rewrite_in_rhs (cR : constr) (tH : constr) : unit :=
+  let goalctx := empty_TEContext cR in 
+  let (goalctx, glhs, grhs) := parse_tensor_equality_aux goalctx (Control.goal()) in 
+  let hypctx := {goalctx with ctx_ml := [] } in 
+  let (hypctx, hlhs, hrhs) := parse_tensor_equality_aux hypctx tH in 
+  let goalml := goalctx.(ctx_ml) in 
+  let ctx := {hypctx with ctx_ml := goalml} in 
+
+  let cgrhs := constr_of_tensorexprdb grhs in 
+  let chlhs := constr_of_tensorexprdb hlhs in 
+  let chrhs := constr_of_tensorexprdb hrhs in 
+  let rew_expr := '(match_rewrite_tensorlist (tensorlist_of_tensorexpr $chlhs) 
+    (tensorlist_of_tensorexpr $chrhs) (tensorlist_of_tensorexpr $cgrhs)) in 
+  let new_rhs_expr := Std.eval_vm None rew_expr in 
+  lazy_match! new_rhs_expr with 
+  | None => Control.zero (Tactic_failure
+    (Some (Message.of_string "te_rewrite_in_rhs: no rewrite found!")))
+  | Some ?e => 
+    let new_rhs_expr := '(tensorexpr_of_tensorlist $e) in 
+    let new_rhs_expr := Std.eval_vm None new_rhs_expr in
+    let new_rhs := tensorexprdb_of_constr new_rhs_expr in
+    let new_goal := constr_semantics_of_tensor_equality ctx glhs new_rhs in 
+    enough ($new_goal) by Control.shelve();
+    red_te_semantics()
+  end.
+
+Ltac2 te_rewrite (cR : constr) (cH : constr) : unit :=
+  let tH := Constr.type cH in 
+  first [te_rewrite_in_lhs cR tH | te_rewrite_in_rhs cR tH].
+
+(*
+(* 
+Ltac2 te_refl parse_abs' : unit :=
+  lazy_match! goal with 
+  | [|- ?_req ?lhs ?rhs] => 
+    let rT := Constr.type lhs in 
+    let sR := get_SRData rT in 
+    let (vs, abs, vars, rels, tel) := parse_tensor_expr_aux_data sR parse_abs'
+      [] (FMap.empty string_tag) (FMap.empty string_tag) []
+      lhs in 
+    let (vs, abs, vars, _rels, ter) := 
+      parse_tensor_expr_aux_data sR parse_abs'
+      vs abs vars rels
+      rhs in 
+
+    let cV := get_cV vs in 
+    let cVsum := get_cVsum vs in 
+    let cabs := constr_of_constr_map constr_of_string
+      (constr_of_typed_fun rT cV)
+      'string '(@Vfunc $rT $cV) 
+      '(gmap string (@Vfunc $rT $cV)) abs in
+
+    let cvars := constr_of_constr_map constr_of_string
+      (fun x => 
+        let (_, tx) := lookup_vs_no_sum vs (Constr.type x) in 
+        let ctx := constr_nat_of_int tx in 
+        '(@mk_Vval $cV $ctx $x)) 'string '(Vval $cV)
+        '(gmap string (Vval $cV)) vars in 
+    
+    let clhs := constr_of_tensorexpr tel in 
+    let crhs := constr_of_tensorexpr ter in 
+    let rSR := sR.(ringSR) in 
+    apply (tensorexpr_eqb_correct_apply (SR:=$rSR)
+      $cV (Vsum:=$cVsum) $cabs $cvars $clhs $crhs);
+    vm_compute;
+    exact eq_refl
+  end.
+
+Ltac2 te_refl_no_check parse_abs' : unit :=
+  lazy_match! goal with 
+  | [|- ?_req ?lhs ?rhs] => 
+    let rT := Constr.type lhs in 
+    let sR := get_SRData rT in 
+    let (vs, abs, vars, rels, tel) := parse_tensor_expr_aux_data sR parse_abs'
+      [] (FMap.empty string_tag) (FMap.empty string_tag) []
+      lhs in 
+    let (vs, abs, vars, _rels, ter) := 
+      parse_tensor_expr_aux_data sR parse_abs'
+      vs abs vars rels
+      rhs in 
+
+    let cV := get_cV vs in 
+    let cVsum := get_cVsum vs in 
+    let cabs := constr_of_constr_map constr_of_string
+      (constr_of_typed_fun rT cV)
+      'string '(@Vfunc $rT $cV) 
+      '(gmap string (@Vfunc $rT $cV)) abs in
+
+    let cvars := constr_of_constr_map constr_of_string
+      (fun x => 
+        let (_, tx) := lookup_vs_no_sum vs (Constr.type x) in 
+        let ctx := constr_nat_of_int tx in 
+        '(@mk_Vval $cV $ctx $x)) 'string '(Vval $cV)
+        '(gmap string (Vval $cV)) vars in 
+    
+    let clhs := constr_of_tensorexpr tel in 
+    let crhs := constr_of_tensorexpr ter in 
+    let rSR := sR.(ringSR) in 
+    apply (tensorexpr_eqb_correct_apply (SR:=$rSR)
+      $cV (Vsum:=$cVsum) $cabs $cvars $clhs $crhs);
+    ltac1:(vm_cast_no_check (@eq_refl bool true))
+  end.
+
+
+Require Import TensorExprFastMatch.
+
+Ltac2 te_refl_fast parse_abs' : unit :=
+  lazy_match! goal with 
+  | [|- ?_req ?lhs ?rhs] => 
+    let rT := Constr.type lhs in 
+    let sR := get_SRData rT in 
+    let (vs, abs, vars, rels, tel) := parse_tensor_expr_aux_data sR parse_abs'
+      [] (FMap.empty string_tag) (FMap.empty string_tag) []
+      lhs in 
+    let (vs, abs, vars, _rels, ter) := 
+      parse_tensor_expr_aux_data sR parse_abs'
+      vs abs vars rels
+      rhs in 
+
+    let cV := get_cV vs in 
+    let cVsum := get_cVsum vs in 
+    let cabs := constr_of_constr_map constr_of_string
+      (constr_of_typed_fun rT cV)
+      'string '(@Vfunc $rT $cV) 
+      '(gmap string (@Vfunc $rT $cV)) abs in
+
+    let cvars := constr_of_constr_map constr_of_string
+      (fun x => 
+        let (_, tx) := lookup_vs_no_sum vs (Constr.type x) in 
+        let ctx := constr_nat_of_int tx in 
+        '(@mk_Vval $cV $ctx $x)) 'string '(Vval $cV)
+        '(gmap string (Vval $cV)) vars in 
+    
+    let clhs := constr_of_tensorexpr tel in 
+    let crhs := constr_of_tensorexpr ter in 
+    let rSR := sR.(ringSR) in 
+    apply (tensorexpr_eqb_correct_apply_db (SR:=$rSR)
+      $cV (Vsum:=$cVsum) $cabs $cvars $clhs $crhs);
+    vm_compute;
+    exact eq_refl
+  end.
+
+Ltac2 te_refl_fast_no_check parse_abs' : unit :=
+  lazy_match! goal with 
+  | [|- ?_req ?lhs ?rhs] => 
+    let rT := Constr.type lhs in 
+    let sR := get_SRData rT in 
+    let (vs, abs, vars, rels, tel) := parse_tensor_expr_aux_data sR parse_abs'
+      [] (FMap.empty string_tag) (FMap.empty string_tag) []
+      lhs in 
+    let (vs, abs, vars, _rels, ter) := 
+      parse_tensor_expr_aux_data sR parse_abs'
+      vs abs vars rels
+      rhs in 
+
+    let cV := get_cV vs in 
+    let cVsum := get_cVsum vs in 
+    let cabs := constr_of_constr_map constr_of_string
+      (constr_of_typed_fun rT cV)
+      'string '(@Vfunc $rT $cV) 
+      '(gmap string (@Vfunc $rT $cV)) abs in
+
+    let cvars := constr_of_constr_map constr_of_string
+      (fun x => 
+        let (_, tx) := lookup_vs_no_sum vs (Constr.type x) in 
+        let ctx := constr_nat_of_int tx in 
+        '(@mk_Vval $cV $ctx $x)) 'string '(Vval $cV)
+        '(gmap string (Vval $cV)) vars in 
+    
+    let clhs := constr_of_tensorexpr tel in 
+    let crhs := constr_of_tensorexpr ter in 
+    let rSR := sR.(ringSR) in 
+    apply (tensorexpr_eqb_correct_apply_db (SR:=$rSR)
+      $cV (Vsum:=$cVsum) $cabs $cvars $clhs $crhs);
+    ltac1:(vm_cast_no_check (@eq_refl bool true))
+  end. *)
+
+
+
+Section Testing.
+
+  Parameter (A : Type).
+  Parameter (SA : Summable A).
+
+  Parameter (B : Type).
+  Parameter (SB : Summable B).
+
+  (* Convertible non-syntactically-equal type *)
+  Definition C := A.
+  Definition SC : Summable C := SA.
+  Typeclasses Opaque C.
+
+  Existing Instance SA.
+  Existing Instance SB.
+  Existing Instance SC.
+
+
+  Context `{SR : SemiRing R rO rI radd rmul req}.
+  Notation "0" := rO.
+  Notation "1" := rI.
+  Notation "x '==' y" := (req x y) (at level 70). 
+  Infix "+" := radd. 
+  Infix "*" := rmul.
+
+
+
+  Parameter (f : A -> B -> A -> R).
+  Parameter (g : A -> B -> R).
+
+  (* #[export] *)
+  (* Hint Extern 0 (ParseAT ?Vs _ _ _ (?f ?a1 ?b2 ?a3)) =>
+    let tA := get_ty_nosum Vs A in 
+    let tB := get_ty_nosum Vs B in 
+    let V := constr:(λ i, projT1 (Vs !!! i)) in
+    notypeclasses refine (Build_ParseAT Vs 
+      (@existT (list Ty) (λ args, V_n_args V args R) 
+        [tA;tB;tA] f : @Vfunc R V)
+      [@mk_Vval V tA a1; @mk_Vval V tB b2] 
+      [@mk_Vval V tA a3] 
+      (f a1 b2 a3) _);
+    constructor; reflexivity : typeclass_instances. *)
+
+  (* #[export] *)
+  (* Hint Extern 0 (ParseAT ?Vs _ _ _ (?g ?a1 ?b2)) =>
+    let tA := get_ty_nosum Vs A in 
+    let tB := get_ty_nosum Vs B in 
+    let V := constr:(λ i, projT1 (Vs !!! i)) in
+    notypeclasses refine (Build_ParseAT Vs 
+      (@existT (list Ty) (λ args, V_n_args V args R) 
+        [tA;tB] g : @Vfunc R V)
+      [@mk_Vval V tA a1] [@mk_Vval V tB b2] 
+      (g a1 b2) _);
+    constructor; reflexivity : typeclass_instances. *)
+
+  Parameter z : A.
+
+  Local Definition te_lhs := 
+    sum_of (fun x : A => sum_of (fun y : B => f x y z * g z y)).
+
+  Local Definition te_rhs := 
+    sum_of (fun y : B => sum_of (fun x : A => g z y * f x y z)).
+
+  Definition te_prob n :=
+    fold_right rmul te_lhs (repeat te_lhs n) == 
+    fold_right rmul te_rhs (repeat te_rhs n).
+
+  Arguments te_lhs /.
+  Arguments te_rhs /.
+  Arguments te_prob /.
+
+  (* Local Ltac te_refl := 
+    unshelve apply (ParseTE_reflexive_test _ _);
+    [..|vm_compute; exact eq_refl];
+    [exact nil|exact gmap_empty|exact gmap_empty]. *)
+
+  (* Set Default Proof Mode "Classic". *)
+
+From Ltac2 Require Import Notations.
+
+Ltac2 Set parse_abstract as parse_abstract_old := fun c relmap => 
+  lazy_match! c with
+  | f ?x ?y ?z => Some ('f, [(x, 'A); (y, 'B)], [(z, 'A)])
+  | g ?x ?y => Some ('g, [(x, 'A)], [(y, 'B)])
+  | _ => parse_abstract_old c relmap
+  end.
+
+
+(* Set Default Proof Mode "Classic". *)
+
+(* Local Ltac2 test (n : int) : unit :=
+  print (of_int n); 
+  let cn := constr_nat_of_int n in 
+  ltac1:(cn |-
+  let H := fresh in 
+  assert (H : te_prob cn) by 
+    ltac2:(cbn; te_refl parse_abs');
+  clear H) (Ltac1.of_constr cn).
+
+Local Ltac2 testf (n : int) : unit :=
+  (* print (of_int n);  *)
+  let cn := constr_nat_of_int n in 
+  let h := Fresh.fresh (Fresh.Free.of_goal ()) ident:(H) in 
+  assert ($h : te_prob $cn) by 
+    (cbn; Control.time (Some (string_of_int n)) 
+      (fun () => (te_refl_fast parse_abs')));
+  clear $h. *)
+
+
+(* Local Ltac2 testfU (n : int) : unit :=
+  (* print (of_int n);  *)
+  let cn := constr_nat_of_int n in 
+  let h := Fresh.fresh (Fresh.Free.of_goal ()) ident:(H) in 
+  assert ($h : te_prob $cn) by 
+    (cbn; Control.time (Some (string_of_int n)) 
+      (fun () => (te_refl_fast_UNSAFE parse_abs')));
+  clear $h. *)
+
+
+
+(*
+Goal True.
+
+test_parse_tensorexpr '(unfolded te_lhs).
+reflexivity.
+
+
+let c := '(unfolded te_lhs == unfolded te_rhs) in 
+let ctx := empty_TEContext 'R in 
+let (ctx, lhs, rhs) := parse_tensor_equality_aux ctx c in 
+let cSR := ctx.(ctx_SR).(ringSR) in 
+let cV := ctx_get_cV ctx in 
+let cVsum := ctx_get_cVsum ctx in 
+let cabs := ctx_get_cabs ctx in 
+let cmg := ctx_get_cmg ctx in 
+let cml := ctx_get_cml_list ctx in 
+let clhs := constr_of_tensorexprdb lhs in 
+let crhs := constr_of_tensorexprdb rhs in 
+(* let clhs := constr_semantics_of_tensorexpr ctx lhs in 
+let crhs := constr_semantics_of_tensorexpr ctx rhs in  *)
+(* let cml := ctx_get_cml ctx in  *)
+assert (@tensorequation_semantics_aux _ _ _ _ _ _ $cSR $cV $cVsum $cabs $cmg [] 
+  $clhs $crhs $cml ∅).
+
+red_te_semantics().
+
+let cR := 'R in 
+let c := '(
+  forall z z', ∑ x : A, ∑ y : B, f x y z * g z' y ==
+   ∑ y : B, ∑ x : A, g z' y * f x y z
+) in 
+Std.resolve_tc c;
+te_rewrite_in_lhs cR c.
+let tH := c in 
+
+  let goalctx := empty_TEContext cR in 
+  let (goalctx, glhs, grhs) := parse_tensor_equality_aux goalctx (Control.goal()) in 
+  let hypctx := {goalctx with ctx_ml := [] } in 
+  let (hypctx, hlhs, hrhs) := parse_tensor_equality_aux hypctx tH in 
+  let goalml := goalctx.(ctx_ml) in 
+  let ctx := {hypctx with ctx_ml := goalml} in 
+
+  let cglhs := constr_of_tensorexprdb glhs in 
+  let chlhs := constr_of_tensorexprdb hlhs in 
+  let chrhs := constr_of_tensorexprdb hrhs in 
+  let rew_expr := '(match_rewrite_tensorlist (tensorlist_of_tensorexpr $chlhs) 
+    (tensorlist_of_tensorexpr $chrhs) (tensorlist_of_tensorexpr $cglhs)) in 
+  let new_lhs_expr := Std.eval_vm None rew_expr in 
+  match! new_lhs_expr with 
+  | None => Control.throw_invalid_argument "te_rewrite_in_lhs: no rewrite found!"
+  | Some ?e => 
+    let new_lhs_expr := '(tensorexpr_of_tensorlist $e) in 
+    let new_lhs_expr := Std.eval_vm None new_lhs_expr in
+    let new_lhs := tensorexprdb_of_constr new_lhs_expr in 
+    let new_goal := constr_semantics_of_tensor_equality ctx new_lhs grhs in 
+    enough ($new_goal) by Control.shelve();
+    red_te_semantics()
+  end.
+
+te_rewrite_in_lhs cR c.
+test_parse_tensor_equality cR c.
+
+
+reflexivity.
+cbn.
+remember @sum_of as s.
+vm_compute.
+subst s.
+
+
+reflexivity.
+vm_compute.
+
+let ctx := empty_TEContext cR in ().
+let (eqctx, lhs, rhs) := parse_tensor_equality_aux ctx tH in ().
+let sem := constr_semantics_of_tensor_equality eqctx lhs rhs in 
+assert ($tH = $sem).
+vm_compute.
+vm_compute (tensorequation_semantics_aux _ _ _ _ _ _).
+cbv beta.
+cbv -[sum_of].
+reflexivity.
+
+(* Ltac2 Eval  *)
+let c := '(unfolded te_lhs == unfolded te_rhs) in 
+let ctx := empty_TEContext 'R in 
+let (ctx, lhs, rhs) := parse_tensor_equality_aux ctx c in 
+let cSR := ctx.(ctx_SR).(ringSR) in 
+let cV := ctx_get_cV ctx in 
+let cVsum := ctx_get_cVsum ctx in 
+let cabs := ctx_get_cabs ctx in 
+let cmg := ctx_get_cmg ctx in 
+let cml := ctx_get_cml_list ctx in 
+let clhs := constr_of_tensorexprdb lhs in 
+let crhs := constr_of_tensorexprdb rhs in 
+(* let clhs := constr_semantics_of_tensorexpr ctx lhs in 
+let crhs := constr_semantics_of_tensorexpr ctx rhs in  *)
+(* let cml := ctx_get_cml ctx in  *)
+'(@tensorequation_semantics_aux _ _ _ _ _ _ $cSR $cV $cVsum $cabs $cmg [] 
+  $clhs $crhs $cml ∅)
+test_parse_tensor_equalitydbR c.
+
+rewrite (unfold te_lhs in te_lhs).
+
+ltac1:(assert (Hrw : forall z w, ∑ x : A, ∑ y : B, f z y x * g x w ==
+g z w) by admit).
+
+Ltac2 Eval 
+  let (ctx, rels, lhs, rhs) := parse_tensor_equality_aux 
+  (empty_TEContext 'R) [] (Constr.type &Hrw) in 
+  (ctx.(ctx_vs), FMap.bindings (ctx.(ctx_vars)), rels, lhs, rhs).
+
+Constr.type 
+
+let cn := constr_nat_of_int 0 in 
+let h := Fresh.fresh (Fresh.Free.of_goal ()) ident:(H) in 
+assert ($h : te_prob $cn).
+cbn.
+
+match! goal with 
+| [|- ?g] => 
+  let ganon := make_binders_anon g in 
+  change $ganon
+end.
+
+
+Ltac2 Eval lazy_match! goal with 
+  | [|- ?_req ?lhs ?rhs] => 
+    let rT := Constr.type lhs in 
+    let sR := get_SRData rT in 
+    let (vs, abs, vars, rels, tel) := parse_tensor_expr_aux_data sR parse_abs'
+      [] (FMap.empty string_tag) (FMap.empty string_tag) []
+      lhs in 
+    tel
+  end.
+
+(* Time test 1.
+Time test 2.
+Time test 3.
+Time test 4.
+Time test 5.
+Time test 6.
+Time test 7.
+Time test 8.
+Time test 9.
+Time test 10.
+Time test 11.
+Time test 12.
+Time test 13.
+Time test 14.
+Time test 15.
+Time test 16.
+Time test 17.
+Time test 18.
+Time test 19.
+Time test 20. *)
+
+
+(* Time testf 1.
+Time testf 2.
+Time testf 3.
+Time testf 4.
+Time testf 5.
+Time testf 6.
+Time testf 7.
+Time testf 8.
+Time testf 9.
+Time testf 10.
+Time testf 11.
+Time testf 12.
+Time testf 13.
+Time testf 14.
+Time testf 15.
+Time testf 16.
+Time testf 17.
+Time testf 18.
+Time testf 19.
+Time testf 20.
+Time testf 21.
+Time testf 22.
+Time testf 23.
+Time testf 24.
+Time testf 25.
+Time testf 26.
+Time testf 27.
+Time testf 28.
+Time testf 29.
+Time testf 30. *)
+(* testf 40.
+testf 50.
+testf 60.
+testf 70.
+testf 80.
+testf 90.
+testf 100.
+testf 40.
+testf 50.
+testf 60.
+testf 70.
+testf 80.
+testf 90.
+testf 100.
+testf 40.
+testf 50.
+testf 60.
+testf 70.
+testf 80.
+testf 90.
+testf 100.
+testf 40.
+testf 50.
+testf 60.
+testf 70.
+testf 80.
+testf 90.
+testf 100.
+testf 40.
+testf 50.
+testf 60.
+testf 70.
+testf 80.
+testf 90.
+testf 100. *)
+
+
+testfU 130.
+testfU 140.
+testfU 150.
+testfU 160.
+testfU 170.
+testfU 180.
+testfU 190.
+testfU 200.
+
+testfU 1.
+testfU 2.
+testfU 3.
+testfU 4.
+testfU 5.
+testfU 6.
+testfU 7.
+testfU 8.
+testfU 9.
+testfU 10.
+testfU 11.
+testfU 12.
+testfU 13.
+testfU 14.
+testfU 15.
+testfU 16.
+testfU 17.
+testfU 18.
+testfU 19.
+testfU 20.
+testfU 21.
+testfU 22.
+testfU 23.
+testfU 24.
+testfU 25.
+testfU 26.
+testfU 27.
+testfU 28.
+testfU 29.
+testfU 30.
+testfU 40.
+testfU 50.
+testfU 60.
+testfU 70.
+testfU 80.
+testfU 90.
+testfU 100.
+testfU 30.
+testfU 40.
+testfU 50.
+testfU 60.
+testfU 70.
+testfU 80.
+testfU 90.
+testfU 100.
+testfU 30.
+testfU 40.
+testfU 50.
+testfU 60.
+testfU 70.
+testfU 80.
+testfU 90.
+testfU 100.
+testfU 30.
+testfU 40.
+testfU 50.
+testfU 60.
+testfU 70.
+testfU 80.
+testfU 90.
+testfU 100.
+testfU 30.
+testfU 40.
+testfU 50.
+testfU 60.
+testfU 70.
+testfU 80.
+testfU 90.
+testfU 100.
+testfU 30.
+testfU 40.
+testfU 50.
+testfU 60.
+testfU 70.
+testfU 80.
+testfU 90.
+testfU 100.
+
+
+(* ltac2:(
+ltac1:(
+let H := fresh in 
+assert (H : let n := 10 in 
+  foldr rmul te_lhs (repeat te_lhs n) == 
+  foldr rmul te_lhs (repeat te_lhs n)));
+cbn). *)
+
+(* Ltac2 Eval (lookup_vs [('A, 'SA); ('B, 'SB)] 'A 'SB). *)
+
+ltac1:(
+let H := fresh in 
+  assert (H : te_prob 20)).
+cbn.
+
+
+(* Time Ltac2 Eval
+lazy_match! goal with 
+| [|- ?_req ?lhs ?rhs] => 
+  let rT := Constr.type lhs in 
+  let sR := get_SRData rT in 
+  let (vs, abs, vars, rels, tel) := parse_tensor_expr_aux sR parse_abs'
+    [] (FMap.empty string_tag) (FMap.empty string_tag) []
+    lhs in 
+  let (vs, abs, vars, rels, ter) := 
+    parse_tensor_expr_aux sR parse_abs'
+    vs abs vars rels
+    rhs in 
+  ter
+end. *)
+
+Time 
+
+(* Time Ltac2 Eval *)
+lazy_match! goal with 
+| [|- ?_req ?lhs ?rhs] => 
+  let rT := Constr.type lhs in 
+  let sR := get_SRData rT in 
+  let (vs, abs, vars, rels, tel) := parse_tensor_expr_aux sR parse_abs'
+    [] (FMap.empty string_tag) (FMap.empty string_tag) []
+    lhs in 
+  let (vs, abs, vars, _rels, ter) := 
+    parse_tensor_expr_aux sR parse_abs'
+    vs abs vars rels
+    rhs in 
+
+  let cV := get_cV vs in 
+  let cVsum := get_cVsum vs in 
+  let cabs := constr_of_constr_map constr_of_string
+    (constr_of_typed_fun rT cV)
+    'string '(@Vfunc $rT $cV) 
+    '(gmap string (@Vfunc $rT $cV)) abs in
+
+  let cvars := constr_of_constr_map constr_of_string
+    (fun x => 
+      let (_, tx) := lookup_vs_no_sum vs (Constr.type x) in 
+      let ctx := constr_nat_of_int tx in 
+      '(@mk_Vval $cV $ctx $x)) 'string '(Vval $cV)
+      '(gmap string (Vval $cV)) vars in 
+(* ()
+end).   *)
+  let clhs := constr_of_tensorexpr tel in 
+  let crhs := constr_of_tensorexpr ter in 
+  let rSR := sR.(ringSR) in 
+  (* let newlhs := '(total_semantics (SR:=$rSR)
+    $cV (Vsum:=$cVsum) $cabs $cvars $clhs) in 
+  let newrhs := '(total_semantics (SR:=$rSR)
+    $cV (Vsum:=$cVsum) $cabs $cvars $crhs) in  *)
+  
+  apply (tensorexpr_eqb_correct_apply_db (SR:=$rSR)
+    $cV (Vsum:=$cVsum) $cabs $cvars $clhs $crhs);
+  vm_compute; exact eq_refl
+  (* ltac1:(vm_cast_no_check (@eq_refl bool true)) *)
+  
+    (* let prf := ('(tensorexpr_eqb_correct_apply (SR:=$rSR)
+    $cV (Vsum:=$cVsum) $cabs $cvars $clhs $crhs 
+      ltac:(vm_cast_no_check (@eq_refl bool true)))) in 
+  
+  (exact $prf)
+   *)
+  
+  
+  (* Control.abstract *)
+  (* let newgoal := '($req $newlhs $newrhs) in *)
+  (* new *)
+  (* ltac1:(prf |- pose proof prf as Heq) (Ltac1.of_constr prf) *)
+  (* Std.vm_cast_no_check prf *)
+    
+  (* change $newgoal;
+  refine '(tensorexpr_eqb_correct_apply (SR:=$rSR)
+    $cV (Vsum:=$cVsum) $cabs $cvars $clhs $crhs _);
+  vm_compute; 
+  exact eq_refl *)
+  (* constr_of_constr_map *)
+  (* constr_of_typed_fun rT cV 
+    (snd (List.nth (FMap.bindings abs) 0)) *)
+  (* (vs, FMap.bindings abs, FMap.bindings vars, rels, te) *)
+  (* constr_of_tensorexpr te *)
+end
+.
+
+Time vm_compute tensorlist_of_tensorexpr.
+Time vm_compute.
+done.
+
+Time vm_compute.
+
+(* From stdpp Require Import sorting.
+Require Import TensorExprFastMatch.
+
+match goal with
+|- context[ tensorlist_of_tensorexpr ?te] => 
+  assert (te_to_tldb te = mk_tldb [] [])
+end.
+1:{ 
+  Time vm_compute.
+}
+
+replace tensorlist_of_tensorexpr with tensorlist_of_tensorexpr_alt_db.
+Time vm_compute tensorlist_of_tensorexpr_alt_db. *)
+
+
+do 2 idtac; [match goal with 
+|- context [tensorlist_of_tensorexpr ?te] => 
+  replace (tensorlist_of_tensorexpr te) with 
+    (tensorlist_of_tensorexpr_alt te)
+end|..].
+2,3: vm_compute; reflexivity.
+
+(* Time vm_compute. *)
+Time vm_compute tensorlist_of_tensorexpr_alt.
+Time vm_compute.
+unfold tensorlist_eqb.
+vm_compute bool_decide at 1.
+cbv match.
+vm_compute canonify_tl_aux''.
+cbv match.
+vm_compute bool_decide at 1.
+cbv match.
+(* Time vm_compute match_tensorlist. *)
+(* Time vm_compute. *)
+Require Import TensorExprFastMatch.
+
+(* Time vm_compute.  *)
+match goal with
+|- context [match_tensorlist ?l ?r] =>
+  replace (match_tensorlist l r) with (match_tensorlist_fast l r) by admit
+end.
+
+Time vm_compute.
+(* Notation "'!Pset' '_'" := (PNodes _) (only printing). *)
+unfold match_tensorlist_fast.
+Time vm_compute list_to_set.
+cbv delta [match_tensorlist_fast_aux] beta.
+Time vm_compute collate.
+Time vm_compute.
+(* rewrite map_fold_foldr. *)
+
+Time vm_compute map_to_list.
+Time vm_compute.
+(* Time vm_compute. *)
+cbv delta [map_fold] beta.
+Pmap_fold
+Time vm_compute map_fold.
+Time vm_compute.
+Time vm_compute match_tensorlist_fast.
+
+(* match goal with 
+|- context [mk_tl _ ?abs] => 
+  match abs with 
+  | merge_sort _ _ => fail 1
+  | _ => 
+  replace abs with 
+    (merge_sort (fun f g => String.le f.1.1 g.1.1) abs) by admit
+  end
+end. *)
+
+do 2 match goal with 
+|- context [mk_tl _ ?abs] => 
+  match abs with 
+  | merge_sort _ _ => fail 1
+  | _ => 
+  replace abs with 
+    (merge_sort (fun f g => lexico f g) abs) by admit
+  end
+end.
+
+vm_compute merge_sort.
+Time vm_compute.
+
+
+evar (tll : tensorlist).
+evar (tlr : tensorlist).
+
+transitivity (tensorlist_eqb tll tlr).
+apply f_equal2.
+
+Time vm_compute; reflexivity.
+Time vm_compute; reflexivity.
+subst tll tlr.
+unfold tensorlist_eqb.
+vm_compute bool_decide at 1.
+cbv match.
+vm_compute canonify_tl_aux''.
+cbv match.
+vm_compute bool_decide at 1.
+cbv match.
+Time vm_compute match_tensorlist at 1.
+Time vm_compute.
+
+match goal with 
+|- context [@bool_decide ?P ?HP] => 
+  vm_compute (@bool_decide P HP)
+end.
+replace (bool_decide _) with true.
+2: vm_compute; reflexivity.
+
+vm_compute (bool_decide _).
+(* replace "f0" with "g". *)
+vm_compute.
+Time vm_compute; reflexivity.
+Time 
+
+
+
+
+match goal with 
+| 
+
+done.
+Time Qed.
+
+Time exact Heq.
+
+
+done.
+(* ltac1:(done). *)
+Time Qed.
+easy.
+
+  
+
+Time te_refl.
+[cbn; time te_refl|clear H].
+]
+cbn.
+Time te_refl.
+
+
+assert (let n := 1%nat in 
+fold_right rmul te_lhs (repeat te_lhs n) == 
+fold_right rmul te_rhs (repeat te_rhs n)).
+cbn. 
+unfold te_lhs, te_rhs.
+Time 
+
+
+
+evar (a : A).
+evar (a' : A).
+evar (a'' : A).
+evar (z : A).
+evar (b : B).
+evar (b' : B).
+evar (b'' : B).
+
+set (te_lhs := sum_of (fun x : A => 
+  sum_of (fun y : B => f x y z * g z y))).
+set (te_rhs := 
+  sum_of (fun y : B => sum_of (fun x : A => g z y * f x y z))).
+
+assert (let n := 1%nat in 
+fold_right rmul te_lhs (repeat te_lhs n) == 
+fold_right rmul te_rhs (repeat te_rhs n)).
+cbn. 
+unfold te_lhs, te_rhs.
+Time 
+unshelve apply (ParseTE_reflexive_test _ _);
+[..|vm_compute; exact eq_refl];
+[exact nil|exact gmap_empty|exact gmap_empty].
+  sum_of (fun x => faaa a'' a' x) * sum_of (fun x : A => faaa a a' a'')).
+Time 
+unshelve apply (ParseTE_reflexive_test _ _);
+[first [exact nil | exact gmap_empty]..|];
+vm_compute; exact eq_refl.
+
+
+(* #[export] *)
+Hint Extern 0 (ParseAT ?Vs _ _ _ (?faab ?a1 ?a2 ?b3)) =>
+  let tA := get_ty_nosum Vs A in 
+  let tB := get_ty_nosum Vs B in 
+  let V := constr:(λ i, projT1 (Vs !!! i)) in
+  notypeclasses refine (Build_ParseAT Vs (@existT (list Ty) (λ args, V_n_args V args R) 
+    [tA;tA;tB] faab : @Vfunc R V)
+    [@mk_Vval V tA a1] [@mk_Vval V tA a2; @mk_Vval V tB b3] 
+    (faab a1 a2 b3) _);
+  constructor; reflexivity : typeclass_instances.
+
+
+
+
+
+Goal True.
+
+evar (a : A).
+evar (a' : A).
+evar (a'' : A).
+evar (b : B).
+evar (b' : B).
+evar (b'' : B).
+
+
+
+
+
+
+
+Parameter (faaa : A -> A -> A -> R).
+Parameter (faab : A -> A -> B -> R).
+Parameter (faba : A -> B -> A -> R).
+Parameter (fabb : A -> B -> B -> R).
+Parameter (fbaa : B -> A -> A -> R).
+Parameter (fbab : B -> A -> B -> R).
+Parameter (fbba : B -> B -> A -> R).
+Parameter (fbbb : B -> B -> B -> R).
+
+
+(* #[export] *)
+Hint Extern 0 (ParseAT ?Vs _ _ _ (?faaa ?a1 ?a2 ?a3)) =>
+  let tA := get_ty_nosum Vs A in 
+  let V := constr:(λ i, projT1 (Vs !!! i)) in
+  notypeclasses refine (Build_ParseAT Vs (@existT (list Ty) (λ args, V_n_args V args R) 
+    [tA;tA;tA] faaa : @Vfunc R V)
+    [@mk_Vval V tA a1] [@mk_Vval V tA a2; @mk_Vval V tA a3] 
+    (faaa a1 a2 a3) _);
+  constructor; reflexivity : typeclass_instances.
+
+(* #[export] *)
+Hint Extern 0 (ParseAT ?Vs _ _ _ (?faab ?a1 ?a2 ?b3)) =>
+  let tA := get_ty_nosum Vs A in 
+  let tB := get_ty_nosum Vs B in 
+  let V := constr:(λ i, projT1 (Vs !!! i)) in
+  notypeclasses refine (Build_ParseAT Vs (@existT (list Ty) (λ args, V_n_args V args R) 
+    [tA;tA;tB] faab : @Vfunc R V)
+    [@mk_Vval V tA a1] [@mk_Vval V tA a2; @mk_Vval V tB b3] 
+    (faab a1 a2 b3) _);
+  constructor; reflexivity : typeclass_instances.
+
+
+
+
+
+Goal True.
+
+evar (a : A).
+evar (a' : A).
+evar (a'' : A).
+evar (b : B).
+evar (b' : B).
+evar (b'' : B).
+
+
+assert ((sum_of (fun x : A => faaa a a' a'' * sum_of (fun x => faaa a'' a' x))) == 
+  sum_of (fun x => faaa a'' a' x) * sum_of (fun x : A => faaa a a' a'')).
+   *)
+
+End Testing.
+*)
