theories/TensorAutomation/TensorExprDBSyntax.v
@@ -1,0 +1,1004 @@
+Require Import Summable.
+Require StringCustomNotation.
+
+From stdpp Require Import strings fin_maps pmap gmap.
+From stdpp Require Import pretty.
+
+Require Import Aux_stdpp.
+
+Definition pos_to_nat_pred (p : positive) : nat :=
+  pred (Pos.to_nat p).
+
+#[local] Coercion pos_to_nat_pred : positive >-> nat.
+
+Definition pos_add_N (p : positive) (n : N) : positive :=
+  match n with
+  | N0 => p
+  | Npos q => Pos.add p q
+  end.
+
+Lemma pos_add_N_to_Z n p : (Zpos (pos_add_N p n) = Zpos p + Z.of_N n)%Z.
+Proof.
+  unfold pos_add_N; destruct n; lia.
+Qed.
+
+
+Definition pos_sub_N (p : positive) (n : N) : positive :=
+  match n with
+  | N0 => p
+  | Npos q => Pos.sub p q
+  end.
+
+Lemma pos_sub_N_to_Z n p : N.lt n (Npos p) ->
+  (Zpos (pos_sub_N p n) = Zpos p - Z.of_N n)%Z.
+Proof.
+  unfold pos_sub_N; destruct n; lia.
+Qed.
+
+(* FIXME: Move *)
+#[global]
+Program Instance Op_pos_to_nat_pred : ZifyClasses.UnOp pos_to_nat_pred :=
+  { TUOp x := (x - 1)%Z }.
+Next Obligation.
+  cbn.
+  unfold pos_to_nat_pred.
+  intros; lia.
+Qed.
+Add Zify UnOp Op_pos_to_nat_pred.
+
+#[global]
+Program Instance Op_pos_add_N : ZifyClasses.BinOp pos_add_N :=
+  { TBOp x y := (x + y)%Z }.
+Next Obligation.
+  cbn.
+  intros.
+  apply pos_add_N_to_Z.
+Qed.
+Add Zify BinOp Op_pos_add_N.
+
+#[global]
+Program Instance Op_pos_sub_N : ZifyClasses.BinOp pos_sub_N :=
+  { TBOp x y := Z.max 1 (x - y)%Z }.
+Next Obligation.
+  cbn.
+  intros.
+  unfold pos_sub_N.
+  destruct m; lia.
+Qed.
+Add Zify BinOp Op_pos_sub_N.
+
+
+(* FIXME: Move *)
+Section lengthN.
+
+Local Open Scope N_scope.
+
+Fixpoint lengthN {A} (l : list A) : N :=
+  match l with
+  | [] => 0%N
+  | _ :: l => N.succ (lengthN l)
+  end.
+Lemma lengthN_correct {A} (l : list A) :
+  N.to_nat (lengthN l) = length l.
+Proof. induction l; cbn; lia. Qed.
+Lemma lengthN_correct_rev {A} (l : list A) :
+  lengthN l = N.of_nat (length l).
+Proof. rewrite <- lengthN_correct; lia. Qed.
+Lemma lengthN_app {A} (l l' : list A) :
+  lengthN (l ++ l') = lengthN l + lengthN l'.
+Proof.
+  now rewrite 3 lengthN_correct_rev, length_app, Nat2N.inj_add.
+Qed.
+
+End lengthN.
+
+
+(* Section TensorExprDB.  *)
+
+Notation Idx := positive.
+  (* Almost all values are [positive]s, as these are more efficient to
+    work with ([Pmap] is much, much faster than [gmap]) *)
+Notation Ty := nat.
+  (* However, types are [nat]s, so that our typing environment can be
+    a list (we will never meaningfully manipulate types anyways) *)
+
+Local Open Scope positive_scope.
+Local Open Scope list_scope.
+
+(* The type of variables in an expression *)
+Inductive var :=
+  | rel : Idx -> var (* A relative/DeBruijn variable, which is summed over *)
+  | loc : Idx -> var (* A variable in the local context
+    (which is semantically universally quantified) *)
+  | glob : Idx -> var. (* A variable in the global context *)
+
+#[export] Instance rel_inj : Inj eq eq rel.
+Proof. congruence. Qed.
+
+#[export] Instance loc_inj : Inj eq eq loc.
+Proof. congruence. Qed.
+
+#[export] Instance glob_inj : Inj eq eq glob.
+Proof. congruence. Qed.
+
+#[export] Instance var_dec : EqDecision var. refine
+  (fun v v' =>
+  match v, v' with
+  | rel r, rel r' =>
+    match Pos.eq_dec r r' with
+    | left Heq => left (f_equal rel Heq)
+    | right Hneq => right (fun Heq => Hneq (rel_inj _ _ Heq))
+    end
+  | loc l, loc l' =>
+    match Pos.eq_dec l l' with
+    | left Heq => left (f_equal loc Heq)
+    | right Hneq => right (fun Heq => Hneq (loc_inj _ _ Heq))
+    end
+  | glob g, glob g' =>
+    match Pos.eq_dec g g' with
+    | left Heq => left (f_equal glob Heq)
+    | right Hneq => right (fun Heq => Hneq (glob_inj _ _ Heq))
+    end
+  | _, _ => right _
+  end); abstract congruence.
+Defined.
+
+#[export] Instance var_countable : Countable var := {
+  encode v := match v with
+    | rel r => r~0~0
+    | loc l => l~1~0
+    | glob g => g~1
+    end%positive;
+  decode p := match p with
+    | r~0~0 => Some (rel r)
+    | l~1~0 => Some (loc l)
+    | g~1 => Some (glob g)
+    | 1 | 2 => None
+    end%positive;
+  decode_encode v :=
+    match v with | rel p | loc p | glob p => eq_refl end
+}.
+
+Definition v2rel (v : var) : option Idx :=
+  match v with
+  | rel r => Some r
+  | _ => None
+  end.
+
+Definition v2loc (v : var) : option Idx :=
+  match v with
+  | loc l => Some l
+  | _ => None
+  end.
+
+Definition v2glob (v : var) : option Idx :=
+  match v with
+  | glob g => Some g
+  | _ => None
+  end.
+
+Definition var_map (fr fl fg : Idx -> Idx) : var -> var :=
+  fun v => match v with
+  | rel r => rel (fr r)
+  | loc l => loc (fl l)
+  | glob g => glob (fg g)
+  end.
+
+Lemma var_map_decomp fr fl fg v :
+  var_map fr fl fg v = default v (((rel ∘ fr) <$> v2rel v) ∪
+    ((loc ∘ fl) <$> v2loc v) ∪
+    ((glob ∘ fg) <$> v2glob v)).
+Proof.
+  now destruct v.
+Qed.
+
+Add Parametric Morphism : var_map with signature
+  (pointwise_relation Idx eq) ==> (pointwise_relation Idx eq) ==>
+  (pointwise_relation Idx eq) ==> (pointwise_relation var eq) as var_map_mor.
+Proof.
+  intros fr fr' Hfr fl fl' Hfl fg fg' Hfg [];
+  cbn; f_equal; auto.
+Qed.
+
+
+Inductive tensorexpr :=
+  | tone : tensorexpr (* The element 1 *)
+  | tabstract (absidx : Idx) (lower : list var) (upper : list var)
+    (* An abstract tensor, indexed by [absidx], with arguments
+      [lower] and [upper] *)
+  | tproduct (l r : tensorexpr) (* The binary product of [tensorexpr]s *)
+  | tsum (ty : Ty) (summand : tensorexpr)
+    (* A sum *).
+
+Definition tabstract' (abs : Idx * list var * list var) : tensorexpr :=
+  let '(abs, lower, upper) := abs in tabstract abs lower upper.
+
+Fixpoint tproducts (tes : list tensorexpr) : tensorexpr :=
+  match tes with
+  | [] => tone
+  | [te] => te
+  | te :: tes => tproduct te (tproducts tes)
+  end.
+
+
+Definition addrel (shift : N) (v : var) : var :=
+  match v with
+  | rel r => rel (pos_add_N r shift)
+  | _ => v
+  end.
+
+Definition withrelshift (shift : N) (f : var -> var) (v : var) : var :=
+  match v with
+  | rel r => if decide (Npos r <= shift)%N then rel r else
+      addrel shift (f (rel (pos_sub_N r shift)))
+  | _ => addrel shift (f v)
+  end.
+
+Add Parametric Morphism : withrelshift with signature
+  eq ==> pointwise_relation var eq ==> pointwise_relation var eq
+  as withrelshift_ext.
+Proof.
+  intros s f f' Hf []; [|cbn; f_equal; apply Hf..].
+  cbn.
+  case_decide; [reflexivity|].
+  f_equal; apply Hf.
+Qed.
+
+Lemma addrel_add s s' v :
+  addrel s (addrel s' v) = addrel (s + s') v.
+Proof.
+  destruct v; cbn; f_equal.
+  lia.
+Qed.
+
+Lemma pos_sub_N_add p n n' :
+  pos_sub_N p (n + n') = pos_sub_N (pos_sub_N p n) n'.
+Proof.
+  unfold N.add; destruct n, n'; cbn; lia.
+Qed.
+
+Lemma withrelshift_add s s' f v :
+  withrelshift s (withrelshift s' f) v = withrelshift (s + s') f v.
+Proof.
+  destruct v; [|cbn; apply addrel_add..].
+  cbn.
+  repeat case_decide; lia || fast_reflexivity || cbn.
+  - f_equal; destruct s; cbn; try lia.
+  - now rewrite addrel_add, pos_sub_N_add.
+Qed.
+
+Fixpoint relabel_te_aux (shift : N) (f : var -> var) (te : tensorexpr) : tensorexpr :=
+  match te with
+  | tone => tone
+  | tabstract absidx lower upper =>
+    tabstract absidx (withrelshift shift f <$> lower)
+      (withrelshift shift f <$> upper)
+  | tproduct l r => tproduct (relabel_te_aux shift f l) (relabel_te_aux shift f r)
+  | tsum ty summand =>
+    tsum ty (relabel_te_aux (N.succ shift) f summand)
+  end.
+
+Add Parametric Morphism s : (relabel_te_aux s) with signature
+  pointwise_relation var eq ==> eq ==> eq as relabel_te_aux_ext.
+Proof.
+  intros f f' Hf te.
+  revert s.
+  induction te; intros s.
+  - reflexivity.
+  - cbn.
+    f_equal; apply list_fmap_ext;
+    intros _ ? _; now apply withrelshift_ext.
+  - cbn.
+    f_equal; auto.
+  - cbn.
+    f_equal; auto.
+Qed.
+
+Definition relabel_te (f : var -> var) (te : tensorexpr) : tensorexpr :=
+  relabel_te_aux 0 f te.
+
+Fixpoint relabel_te_alt (f : var -> var) (te : tensorexpr) : tensorexpr :=
+  match te with
+  | tone => tone
+  | tabstract absidx lower upper =>
+    tabstract absidx (f <$> lower) (f <$> upper)
+  | tproduct l r => tproduct (relabel_te_alt f l) (relabel_te_alt f r)
+  | tsum ty summand =>
+    tsum ty (relabel_te_alt (withrelshift 1 f) summand)
+  end.
+
+
+Add Parametric Morphism : relabel_te_alt with signature
+  pointwise_relation var eq ==> eq ==> eq as relabel_te_alt_ext.
+Proof.
+  intros f f' Hf te.
+  revert f f' Hf;
+  induction te; intros f f' Hf.
+  - reflexivity.
+  - cbn.
+    f_equal; apply list_fmap_ext;
+    intros _ ? _; now apply Hf.
+  - cbn.
+    f_equal; auto.
+  - cbn.
+    f_equal.
+    apply IHte.
+    now apply withrelshift_ext.
+Qed.
+
+Lemma relabel_te_alt_correct_aux shift f te :
+  relabel_te_alt (withrelshift shift f) te =
+  relabel_te_aux shift f te.
+Proof.
+  revert shift f; induction te; intros shift f.
+  - reflexivity.
+  - reflexivity.
+  - cbn.
+    f_equal; auto.
+  - cbn.
+    rewrite <- IHte.
+    f_equal.
+    apply relabel_te_alt_ext; [|easy].
+    intros v.
+    rewrite withrelshift_add.
+    apply withrelshift_ext; easy + lia.
+Qed.
+
+
+
+
+Fixpoint te_varset (te : tensorexpr) : gset var :=
+  match te with
+  | tone => ∅
+  | tabstract _ lower upper => list_to_set (lower ++ upper)
+  | tproduct l r => te_varset l ∪ te_varset r
+  | tsum ty summand =>
+    te_varset summand
+  end.
+
+(* FIXME: Move *)
+(* The predicate determining that a [tensorexpr] is well-typed
+  _only with respect to bound [rel] variables_ *)
+Fixpoint te_wellbound_aux (bnd : Idx) (te : tensorexpr) : bool :=
+  match te with
+  | tone => true
+  | tabstract _ low up =>
+    bool_decide (Forall (λ p, p < bnd) (omap v2rel (low ++ up)))
+  | tproduct l r => te_wellbound_aux bnd l && te_wellbound_aux bnd r
+  | tsum _ smd =>
+    te_wellbound_aux (Pos.succ bnd) smd
+  end.
+
+Definition te_wellbound (te : tensorexpr) : bool :=
+  te_wellbound_aux 1 te.
+
+
+Fixpoint te_rel_varset (te : tensorexpr) : Pset :=
+  match te with
+  | tone => ∅
+  | tabstract _ lower upper => list_to_set (omap v2rel (lower ++ upper))
+  | tproduct l r => te_rel_varset l ∪ te_rel_varset r
+  | tsum _ smd =>
+    te_rel_varset smd
+  end.
+
+Fixpoint te_local_varset (te : tensorexpr) : Pset :=
+  match te with
+  | tone => ∅
+  | tabstract _ lower upper => list_to_set (omap v2loc (lower ++ upper))
+  | tproduct l r => te_local_varset l ∪ te_local_varset r
+  | tsum _ smd =>
+    te_local_varset smd
+  end.
+
+Fixpoint te_global_varset (te : tensorexpr) : Pset :=
+  match te with
+  | tone => ∅
+  | tabstract _ lower upper => list_to_set (omap v2glob (lower ++ upper))
+  | tproduct l r => te_global_varset l ∪ te_global_varset r
+  | tsum _ smd =>
+    te_global_varset smd
+  end.
+
+Fixpoint te_absset (te : tensorexpr) : Pset :=
+  match te with
+  | tone => ∅
+  | tabstract idx _ _ => {[ idx ]}
+  | tproduct l r => te_absset l ∪ te_absset r
+  | tsum _ summand =>
+    te_absset summand
+  end.
+
+
+Lemma te_varset_decomp te :
+  te_varset te = set_map rel (te_rel_varset te) ∪
+    set_map loc (te_local_varset te) ∪
+    set_map glob (te_global_varset te).
+Proof.
+  unfold_leibniz.
+  induction te; cbn in *; [set_solver| |
+    rewrite 1?IHte1, 1?IHte2; set_solver +|apply IHte].
+  generalize (lower ++ upper) as l.
+  intros l; induction l as [|[]]; [set_solver|
+    cbn [list_to_set omap list_omap v2rel v2loc v2glob];
+  rewrite IHl; set_solver+..].
+Qed.
+
+
+
+
+
+
+
+Record tensorlist := mk_tl {
+  tl_sums : list Ty;
+  tl_abstracts : list (Idx * list var * list var)
+}.
+
+Lemma tl_ext tl tl' :
+  tl.(tl_sums) = tl'.(tl_sums) ->
+  tl.(tl_abstracts) = tl'.(tl_abstracts) ->
+  tl = tl'.
+Proof.
+  destruct tl, tl'; cbn; congruence.
+Qed.
+
+Definition tl_cons_sum ty (tl : tensorlist) : tensorlist :=
+  mk_tl (ty :: tl.(tl_sums)) (tl.(tl_abstracts)).
+
+Fixpoint tl_app_sums sums tl :=
+  match sums with
+  | [] => tl
+  | ty :: sums => tl_cons_sum ty (tl_app_sums sums tl)
+  end.
+
+Fixpoint tensorexpr_of_tensorlist_aux sums abs : tensorexpr :=
+  match sums with
+  | [] => tproducts (tabstract' <$> abs)
+  | ty :: sums => tsum ty (tensorexpr_of_tensorlist_aux sums abs)
+  end.
+
+Definition tensorexpr_of_tensorlist (tl : tensorlist) : tensorexpr :=
+  tensorexpr_of_tensorlist_aux (tl.(tl_sums)) (tl.(tl_abstracts)).
+
+Coercion tensorexpr_of_tensorlist : tensorlist >-> tensorexpr.
+
+
+Definition tlone : tensorlist := mk_tl [] [].
+
+Lemma tlone_correct : tlone =@{tensorexpr} tone.
+Proof.
+  reflexivity.
+Qed.
+
+
+Definition tensorlist_perm_eq (tl tl' : tensorlist) :=
+  tl.(tl_sums) ≡ₚ tl'.(tl_sums) /\
+  tl.(tl_abstracts) ≡ₚ tl'.(tl_abstracts).
+
+
+(* Variable sets for [tensorlist]s *)
+
+Definition abstracts_vars (abs : list (Idx * list var * list var)) : gset var :=
+  list_to_set ('(_, lower, upper) ← abs; lower ++ upper).
+
+Definition abstracts_rel_vars
+  (abs : list (Idx * list var * list var)) : Pset :=
+  list_to_set ('(_, lower, upper) ← abs; omap v2rel (lower ++ upper)).
+
+Definition abstracts_local_vars
+  (abs : list (Idx * list var * list var)) : Pset :=
+  list_to_set ('(_, lower, upper) ← abs; omap v2loc (lower ++ upper)).
+
+Definition abstracts_global_vars
+  (abs : list (Idx * list var * list var)) : Pset :=
+  list_to_set ('(_, lower, upper) ← abs; omap v2glob (lower ++ upper)).
+
+
+
+
+(** Relabeling in [tensorlist]s *)
+
+Definition relabel_abs (f : var -> var) (abs : Idx * list var * list var) :=
+  let '(idx, lower, upper) := abs in
+  (idx, f <$> lower, f <$> upper).
+
+Definition relabel_tl (f : var -> var) (tl : tensorlist) : tensorlist :=
+  mk_tl (tl.(tl_sums))
+    (relabel_abs f <$> tl.(tl_abstracts)).
+
+Definition relabel_rels (f : Idx -> Idx) : var -> var :=
+    var_map f id id.
+
+
+(* A simpler, but less performant, definition *)
+Definition tl_times_spec_defn (l r : tensorlist) : tensorlist :=
+  let 'mk_tl lsums labs := l in
+  let 'mk_tl rsums rabs := r in
+  let lenl := length lsums in
+  let lenr := length rsums in
+  let labs' := relabel_abs (relabel_rels
+    (λ p, pos_add_N p (N.of_nat lenr))) <$> labs in
+  let rabs' := relabel_abs (relabel_rels (λ p,
+    if decide (p < lenr)%nat then p
+    else pos_add_N p (N.of_nat lenl))) <$> rabs in
+  mk_tl (lsums ++ rsums) (labs' ++ rabs').
+
+
+Definition tl_times (l r : tensorlist) : tensorlist :=
+  let 'mk_tl lsums labs := l in
+  let 'mk_tl rsums rabs := r in
+  let lenl := lengthN lsums in
+  let lenr := lengthN rsums in
+  let labs' := match lenr with
+    | N0 => labs
+    | Npos lenr => relabel_abs (relabel_rels (Pos.add lenr)) <$> labs
+    end in
+  let rabs' := match lenl with
+    | N0 => rabs
+    | Npos lenl => match lenr with
+      | N0 => relabel_abs (relabel_rels (Pos.add lenl)) <$> rabs
+      | Npos lenr => relabel_abs (relabel_rels (λ p,
+        if Pos.leb p lenr then p else Pos.add lenl p)) <$> rabs
+      end
+    end in
+  mk_tl (lsums ++ rsums) (labs' ++ rabs').
+
+
+(* FIXME: Move *)
+Lemma list_fmap_id' `(f : A -> A) (l : list A) :
+  (forall a, a ∈ l -> f a = a) ->
+  f <$> l = l.
+Proof.
+  intros Hf.
+  etransitivity; [|apply list_fmap_id].
+  apply list_fmap_ext; intros _ ? ?%elem_of_list_lookup_2.
+  now apply Hf.
+Qed.
+
+Ltac tspecialize_with C tac :=
+  match type of C with
+  | forall _ : ?A, _ =>
+    let H := fresh in
+    assert (H : A); [
+      tac | specialize (C H); clear H
+    ]
+  end.
+
+Tactic Notation "tspecialize" uconstr(C) "by" tactic3(tac) :=
+  tspecialize_with C ltac:(solve [tac]).
+
+Tactic Notation "tspecialize" uconstr(C) :=
+  tspecialize_with C ltac:(idtac).
+
+#[local] Coercion N.of_nat : nat >-> N.
+
+Lemma relabel_abs_id abs : relabel_abs id abs = abs.
+Proof.
+  destruct abs as [[f low] up]; cbn.
+  now rewrite 2 list_fmap_id.
+Qed.
+
+Lemma relabel_abs_ext f g abs :
+  (forall x, f x = g x) -> relabel_abs f abs = relabel_abs g abs.
+Proof.
+  intros Heq.
+  destruct abs as [[idx low] up]; cbn.
+  f_equal; [f_equal|]; apply list_fmap_ext; intros; apply Heq.
+Qed.
+
+Lemma relabel_abs_id' f abs :
+  (forall x, f x = x) -> relabel_abs f abs = abs.
+Proof.
+  intros Hid.
+  erewrite relabel_abs_ext; [apply relabel_abs_id|apply Hid].
+Qed.
+
+Lemma relabel_rels_ext f g :
+  (forall r, f r = g r) -> forall v, relabel_rels f v = relabel_rels g v.
+Proof.
+  intros Hfg.
+  destruct v; [|reflexivity..].
+  cbn; now rewrite Hfg.
+Qed.
+
+
+Lemma tl_times_spec_defn_correct l r :
+  tl_times l r = tl_times_spec_defn l r.
+Proof.
+  destruct l as [lsums labs], r as [rsums rabs].
+  cbn.
+  rewrite <- !lengthN_correct_rev, <- !lengthN_correct.
+  f_equal; f_equal.
+  - case_match eqn:Hrsums.
+    + cbn.
+      symmetry.
+      apply list_fmap_id'.
+      intros; apply relabel_abs_id'.
+      now intros [].
+    + apply list_fmap_ext; intros _ ? _.
+      apply relabel_abs_ext; intros []; [cbn; now rewrite Pos.add_comm|
+        reflexivity..].
+  - destruct (lengthN lsums) as [|lenl] eqn:Hlsums;
+    [|destruct (lengthN rsums) as [|lenr] eqn:Hrsums].
+    + cbn.
+      symmetry.
+      apply list_fmap_id'.
+      intros; apply relabel_abs_id'.
+      now intros []; cbn; [case_match|..].
+    + apply list_fmap_ext; intros _ ? _.
+      apply relabel_abs_ext; intros []; [cbn; now rewrite Pos.add_comm|
+        reflexivity..].
+    + apply list_fmap_ext; intros _ ? _.
+      apply relabel_abs_ext.
+      intros [p| |]; [|reflexivity..].
+      cbn.
+      destruct (Pos.leb_spec p lenr);
+      [rewrite decide_True by lia|rewrite decide_False by lia];
+      f_equal; lia.
+Qed.
+
+
+
+(** Converting a [tensorexpr] to a [tensorlist] *)
+
+Fixpoint tensorlist_of_tensorexpr (te : tensorexpr) : tensorlist :=
+  match te with
+  | tone => tlone
+  | tabstract idx lower upper => mk_tl [] [(idx, lower, upper)]
+  | tproduct l r => tl_times (tensorlist_of_tensorexpr l) (tensorlist_of_tensorexpr r)
+  | tsum ty smd =>
+    tl_cons_sum ty (tensorlist_of_tensorexpr smd)
+  end.
+
+
+
+(* Matching on [tensorlist]s *)
+
+
+(* TO DO: When I figure out the "boundary condition" or whatever that is,
+   incorporate it into the function at this level somehow? *)
+(* TODO: Figure out incorporating typing into this!! As-is this will be 
+  hard to reason about without WF conditions*)
+  (* TODO: Why do I hate WF conditions? TODO: Do I hate WF conditions? 
+    Checking it is probably a pretty small price to pay... especially at
+    the tensorlist level*)
+Fixpoint extend_map_of_abstract_pair
+  (mb mbi : Pmap Idx) (* The map and inverse map of [rel]/bound variables, 
+    which must map to other bound variables *)
+  (ml : Pmap var) (* The map of local variables, which can map to any [var] *)
+  (mlran : Pset) (* The set of [rel] variables in the range of [ml], which
+     must be disjoint from the image of [mb] / domain of [mbi] *)
+  (l r : list var) : option (Pmap Idx * Pmap Idx * Pmap var) :=
+  match l, r with
+  | [], [] => Some (mb, mbi, ml)
+  | hl :: l, hr :: r =>
+    match hl, hr with
+    | glob gl, glob gr => (* global variables must match exactly! *)
+      if bool_decide (gl = gr) then
+        extend_map_of_abstract_pair mb mbi ml mlran l r
+      else None
+    | glob gl, _ => (* global variables can't map anywhere (nontrivially) *)
+      None
+    | loc ll, vr => (* local variables can map anywhere (ab initio, at least) *)
+      match ml !! ll with
+      | None => 
+        match vr with 
+        | rel rr => 
+          match mbi !! rr with
+          | Some _ => None (* This variable is already bound; we can't use it locally *)
+          | None =>
+            extend_map_of_abstract_pair mb mbi (<[ll := rel rr]> ml) ({[rr]} ∪ mlran) 
+              l r
+          end
+        | vr => 
+          extend_map_of_abstract_pair mb mbi (<[ll := vr]> ml) mlran l r
+        end
+      | Some vr' =>
+        if bool_decide (vr = vr') then
+          extend_map_of_abstract_pair mb mbi ml mlran l r
+        else None
+      end
+    | rel rl, rel rr => (* bound variables must map to bound variables *)
+      match mb !! rl with
+      | None => 
+        match mbi !! rr with (* Preserve the inverses! *)
+        | None => 
+          if bool_decide (rr ∈ mlran) then 
+            (* This relative variable is mapped to by a local variable already *)
+            None 
+          else 
+            extend_map_of_abstract_pair 
+              (<[rl := rr]> mb) (<[rr := rl]> mbi) ml mlran l r
+        | Some _ => None (* This variable is already mapped to *)
+        end
+      | Some rr' =>
+        if bool_decide (rr = rr') then
+          extend_map_of_abstract_pair mb mbi ml mlran l r
+        else None
+      end
+    | rel rl, _ => (* bound variables can only map to other bound variables *)
+      None
+    end
+  | _, _ => None
+  end.
+
+(* FIXME: Move *)
+Definition list_first_omap {A B} (f : A -> option B) : list A -> option B :=
+  fix list_first_omap l :=
+  match l with
+  | [] => None
+  | a :: l =>
+    match f a with
+    | Some b => Some b
+    | None => list_first_omap l
+    end
+  end.
+
+
+(* TODO: rewrite with collate (also, optionally shortcut to false if
+  we don't use up all the abstracts for a given index) *)
+Fixpoint extend_match_of_abstract_tensors
+  (P : Pmap Idx -> Pmap Idx -> Pmap var -> Pset -> 
+    list (Idx * list var * list var) -> Prop)
+  `{HP : forall mb mbi ml mlran rrest, Decision (P mb mbi ml mlran rrest)}
+  (mb mbi : Pmap Idx) (* The map and inverse map of [rel]/bound variables, 
+    which must map to other bound variables *)
+  (ml : Pmap var) (* The map of local variables, which can map to any [var] *)
+  (mlran : Pset) (* The set of [rel] variables in the range of [ml], which
+     must be disjoint from the image of [mb] / domain of [mbi] *)
+  (labs rabs : list (Idx * list var * list var)) :
+    option (Pmap Idx * Pmap Idx * Pmap var * Pset * list (Idx * list var * list var)) :=
+  match labs with
+  | [] =>
+    if decide (P mb mbi ml mlran rabs) then
+      Some (mb, mbi, ml, mlran, rabs)
+    else None
+  | (fl, lowl, upl) :: labs =>
+    list_first_omap (fun '((_, lowr, upr), rrest) =>
+      '(mb, mbi, ml) ← extend_map_of_abstract_pair mb mbi ml mlran lowl lowr;
+         '(mb, mbi, ml) ← extend_map_of_abstract_pair mb mbi ml mlran upl upr;
+        extend_match_of_abstract_tensors P mb mbi ml mlran labs rrest)
+      (list_select (fun '(fr, _, _) => fl = fr) rabs)
+    (* head ('((_, lowr, upr), rrest) ← list_select (fun '(fr, _, _) => fl = fr) rabs;
+      from_option (λ x, [x]) []
+        (m' ← extend_map_of_abstract_pair lbound rbound m lowl lowr;
+         m'' ← extend_map_of_abstract_pair lbound rbound m' upl upr;
+         extend_match_of_abstract_tensors lbound rbound m'' labs rrest)
+      ) *)
+  end.
+
+(* TODO: Theory of: 
+Definition lookup _ endomorphism `{Lookup A A M} (m : M) : A -> A :=
+  fun a => default a (m !! a). *)
+
+(* FIXME: Move *)
+Definition Pmap_map (m : Pmap Idx) : Idx -> Idx :=
+  fun v => default v (m !! v).
+
+Definition match_tensorlist_aux (tl tl' : tensorlist) : 
+  option (tensorlist * (* What remains of [tl'] after the match of [tl] is removed *)
+  Pmap Idx * (* The mapping of _unmatched_ bound variables from the unmatched
+    portion of [tl'] to those in the returned tensorlist *)
+  Pmap var) (* The mapping of the local variables of [tl] to variables of
+    [tl'], possibly including relative variables (which are reindexed to
+      be correct within the returned tensorlist; however, they must be 
+      shifted along with the variables of the abstracts of the returned
+      tensorlist if (innermost) sums are added to the tensorlist) *) :=
+  match extend_match_of_abstract_tensors
+    (fun mb mbi ml mlran rabs => 
+      (* TODO: Check this progressively, using [collate] *)
+      set_Forall (λ r, ~ is_Some (mbi !! r)) (abstracts_rel_vars rabs))
+    ∅ ∅ ∅ ∅ (tl.(tl_abstracts)) (tl'.(tl_abstracts)) with 
+  | None => None
+  | Some (mb, mbi, ml, mlran, rrest) =>
+  
+  (* We have: [mb/mbi] : maps [Idx -> Idx] such that 
+    [mb <$> tl] is a subexpression of [tl']; notably:
+    (i) the sums not included in [mb <$> tl] are those of [tl'] 
+      that are _not_ included in [img mb = dom mbi]
+    (ii) the abstracts not included in [mb <$> tl] are [rrest] 
+    
+    We need two maps [reord reord_rest : Idx -> Idx] such that
+    [reord_rest <$> rrest] makes the variables correct there, assuming
+    we simply remove the match (we also need to figure out the order of 
+    types; same thing), and such that [reord]
+    *)
+  Some (
+  let ntys := imap (fun i ty => (Pos.of_succ_nat i, ty)) (reverse tl'.(tl_sums)) in 
+  let unused_tys := filter (fun '(idx, _) => ~ is_Some (mbi !! idx)) ntys in 
+  let newty_info := imap (fun inew '(iold, ty) => (iold, Pos.of_succ_nat inew, ty)) unused_tys in 
+  let rrest_map : Pmap _ := list_to_map newty_info.*1 in 
+  let newtys := reverse newty_info.*2 in 
+  let ml' := (relabel_rels (Pmap_map rrest_map) <$> ml) in
+  (mk_tl newtys (relabel_abs (relabel_rels (Pmap_map rrest_map)) <$> 
+    rrest),
+  rrest_map, ml'))
+  end.
+
+Definition var_subst_locals (f : Idx -> var) (v : var) : var :=
+  match v with 
+  | loc l => f l
+  | _ => v
+  end.
+
+(* TODO: Definitely need to make sure [ml] maps locals to variables 
+  of the correct type. Can do this with overall WF of goal (can get 
+  all typing from the abstract map, then check; if [lhs == rhs] not
+  WF, we should still maybe be fine? I'd thought this worked before
+  but now I'm not positive). *)
+
+(* Assuming [lhs == rhs] (for the moment, ignore typing and context),
+  rewrite this equality in [targ], if possible. *)
+Definition match_rewrite_tensorlist (lhs rhs targ : tensorlist) : 
+  option tensorlist := 
+  '((mk_tl usums uabs), relmap, locmap) ← match_tensorlist_aux lhs targ;
+  let '(mk_tl rsums rabs) := rhs in 
+  let rsize := lengthN rsums in 
+  let shift := relabel_rels (λ p, pos_add_N p rsize) in 
+  let uabs_shifted := relabel_abs shift <$> uabs in 
+  let rabs_subst := relabel_abs (var_subst_locals (λ l, 
+    from_option shift (loc l) (locmap !! l))) <$> rabs in 
+  Some (mk_tl (usums ++ rsums) (uabs_shifted ++ rabs_subst)).
+
+
+
+(* 
+
+Record namedtensorlist := mk_ntl {
+  ntl_sums : list (Idx * Ty);
+  ntl_abstracts : list (Idx * list var * list var);
+}.
+
+
+Definition ntl2tl (ntl : namedtensorlist) :=
+  let '(mk_ntl sums abs) := ntl in 
+  let varmap : Pmap Idx := list_to_map 
+    (imap (λ idx '(r, ty), (r, Pos.of_succ_nat idx))
+      sums) in
+  mk_tl sums.*2
+  (relabel_abs (relabel_rels (λ v, default v (varmap !! v))) <$> abs).
+
+Definition tl2ntl (tl : tensorlist) := 
+  let '(mk_tl sums abs) := tl in 
+  mk_ntl (imap (λ i v, (Pos.of_succ_nat i, v)) (reverse sums))
+    abs.
+
+Definition WF_ntl (ntl : namedtensorlist) : Prop :=
+  NoDup ntl.(ntl_sums).*1 /\
+  abstracts_rel_vars ntl.(ntl_abstracts) ⊆ list_to_set ntl.(ntl_sums).*1.
+
+Definition WF_tl (tl : tensorlist) : Prop :=
+  set_Forall (fun k => (k < Pos.of_succ_nat (length tl.(tl_sums))))
+  (abstracts_rel_vars tl.(tl_abstracts)).
+
+(* Definition match_tensorlist_eq (tl tl' : tensorlist) :
+  option (Pmap Idx * Pmap Idx * Pmap var * Pset * list (Idx * list var * list var)) :=
+  extend_match_of_abstract_tensors
+    (fun mb mbi ml mlran rabs => rabs = [])
+    ∅ ∅ ∅ ∅ (tl.(tl_abstracts)) (tl'.(tl_abstracts)). *)
+
+Definition make_match_namedtensorlist_data 
+  (rsums : list (Idx * Ty)) (rabs : list _) 
+  (mbi : Pmap Idx) : namedtensorlist :=
+  mk_ntl (filter (λ '(idx, ty), ~ is_Some (mbi !! idx)) rsums) rabs.
+
+Definition match_namedtensorlist_aux (tl tl' : namedtensorlist) :
+  option (namedtensorlist * Pmap Idx * Pmap Idx * Pmap var * Pset) :=
+  '(mb, mbi, ml, mlran, rrest) ← extend_match_of_abstract_tensors
+    (fun mb mbi ml mlran rabs => 
+      set_Forall (λ r, ~ is_Some (mbi !! r)) (abstracts_rel_vars rabs))
+    ∅ ∅ ∅ ∅ (tl.(ntl_abstracts)) (tl'.(ntl_abstracts));
+  Some (make_match_namedtensorlist_data tl'.(ntl_sums) rrest mbi, 
+    mb, mbi, ml, mlran).
+
+Definition match_rewrite_namedtensorlist (lhs rhs target : namedtensorlist) : 
+  option namedtensorlist :=
+  '() match_namedtensorlist_aux lhs target with 
+  | None => None
+  | (* TODO: Problem!!! Here, I want to insert the rhs—but the bound variables
+    could conflict! I want to work only with WF namedtensorlist, so this is 
+    actually a big problem. (Un)Fortunately, there's a simple solution: I just
+    need to work with [tensorlist]s exclusively (yes, with all the relabeling
+    hell that will create). I believe the algorithm should be essentially the
+    same, and we'll do much the same as [ntl2tl] to do the renumbering
+    (i.e., [imap] is the key) *) MThrow
+
+Definition match_tensorlist *)
+
+
+
+(* OLD: 
+
+(* Matching on [tensorlist]s *)
+
+(* TODO: When I figure out the "boundary condition" or whatever that is,
+   incorporate it into the function at this level somehow? *)
+Fixpoint extend_map_of_abstract_pair
+  (mb : Pmap Idx) (* The map of [rel]/bound variables, which must map
+    to other bound variables *)
+  (ml : Pmap var) (* The map of local variables, which can map to any [var] *)
+  (l r : list var) : option (Pmap Idx * Pmap var) :=
+  match l, r with
+  | [], [] => Some (mb, ml)
+  | hl :: l, hr :: r =>
+    match hl, hr with
+    | glob gl, glob gr => (* global variables must match exactly! *)
+      if bool_decide (gl = gr) then
+        extend_map_of_abstract_pair mb ml l r
+      else None
+    | glob gl, _ => (* global variables can't map anywhere (nontrivially) *)
+      None
+    | loc ll, vr => (* local variables can map anywhere (ab initio, at least) *)
+      match ml !! ll with
+      | None => extend_map_of_abstract_pair mb (<[ll := vr]> ml) l r
+      | Some vr' =>
+        if bool_decide (vr = vr') then
+          extend_map_of_abstract_pair mb ml l r
+        else None
+      end
+    | rel rl, rel rr => (* bound variables must map to bound variables *)
+      match mb !! rl with
+      | None => extend_map_of_abstract_pair (<[rl := rr]> mb) ml l r
+      | Some rr' =>
+        if bool_decide (rr = rr') then
+          extend_map_of_abstract_pair mb ml l r
+        else None
+      end
+    | rel rl, _ => (* bound variables can only map to other bound variables *)
+      None
+    end
+  | _, _ => None
+  end.
+
+Definition list_first_omap {A B} (f : A -> option B) : list A -> option B :=
+  fix list_first_omap l :=
+  match l with
+  | [] => None
+  | a :: l =>
+    match f a with
+    | Some b => Some b
+    | None => list_first_omap l
+    end
+  end.
+
+
+(* TODO: rewrite with collate (also, optionally shortcut to false if
+  we don't use up all the abstracts for a given index) *)
+Fixpoint extend_match_of_abstract_tensors
+  (P : Pmap Idx -> Pmap var -> list (Idx * list var * list var) -> Prop)
+  `{HP : forall mb ml rrest, Decision (P mb ml rrest)}
+  (mb : Pmap Idx) (* The map of [rel]/bound variables, which must map
+    to other bound variables *)
+  (ml : Pmap var) (* The map of local variables, which can map to any [var] *)
+  (labs rabs : list (Idx * list var * list var)) :
+    option (Pmap Idx * Pmap var * list (Idx * list var * list var)) :=
+  match labs with
+  | [] =>
+    if decide (P mb ml rabs) then
+      Some (mb, ml, rabs)
+    else None
+  | (fl, lowl, upl) :: labs =>
+    list_first_omap (fun '((_, lowr, upr), rrest) =>
+      '(mb, ml) ← extend_map_of_abstract_pair mb ml lowl lowr;
+         '(mb, ml) ← extend_map_of_abstract_pair mb ml upl upr;
+        extend_match_of_abstract_tensors P mb ml labs rrest)
+      (list_select (fun '(fr, _, _) => fl = fr) rabs)
+    (* head ('((_, lowr, upr), rrest) ← list_select (fun '(fr, _, _) => fl = fr) rabs;
+      from_option (λ x, [x]) []
+        (m' ← extend_map_of_abstract_pair lbound rbound m lowl lowr;
+         m'' ← extend_map_of_abstract_pair lbound rbound m' upl upr;
+         extend_match_of_abstract_tensors lbound rbound m'' labs rrest)
+      ) *)
+  end.
+
+Definition match_tensorlist (tl tl' : tensorlist) :
+  option (Pmap Idx * Pmap var * list (Idx * list var * list var)) :=
+  extend_match_of_abstract_tensors
+    (fun mb ml rabs => rabs = [])
+    ∅ ∅ (tl.(tl_abstracts)) (tl'.(tl_abstracts)).
+
+
+*)
+
+
