theories/TensorAutomation/Utility/ConstrExtra.v
@@ -1,0 +1,186 @@
+Require Import Ltac2.Init.
+From Ltac2 Require Export Constr.
+Require Ltac2.List.
+Require Ltac2.Fresh.
+Require Ltac2.Std.
+Require PrintingExtra.
+
+
+Import Unsafe.
+
+Local Ltac2 map_invert (f : constr -> constr) (iv : case_invert) : case_invert :=
+  match iv with
+  | NoInvert => NoInvert
+  | CaseInvert indices => CaseInvert (Array.map f indices)
+  end.
+
+(** [map_with_binders_alt g f n c] maps [f n] on the immediate subterms of [c];
+   it carries an extra data [n] (typically a lift index) which is processed by [g]
+   (which typically add 1 to [n]) at each binder traversal;
+   it is not recursive and the order with which subterms are processed is not specified. *)
+Ltac2 map_with_binders_alt 
+  (lift : 'a -> binder -> binder * 'a) 
+  (f : 'a -> constr -> constr) (n : 'a) (c : constr) : constr :=
+  match kind c with
+  | Rel _ | Meta _ | Var _ | Sort _ | Constant _ _ | Ind _ _
+  | Constructor _ _ | Uint63 _ | Float _ | String _ => c
+  | Cast c k t =>
+      let c := f n c
+      with t := f n t in
+      make (Cast c k t)
+  | Prod b c =>
+      let (b, n) := lift n b in
+      let c := f n c in
+      make (Prod b c)
+  | Lambda b c =>
+      let (b, n) := lift n b in
+      let c := f n c in
+      make (Lambda b c)
+  | LetIn b t c =>
+      let t := f n t in 
+      let (b, n) := lift n b in
+      let c := f n c in
+      make (LetIn b t c)
+  | App c l =>
+      let c := f n c
+      with l := Array.map (f n) l in
+      make (App c l)
+  | Evar e l =>
+      let l := Array.map (f n) l in
+      make (Evar e l)
+  | Case info x iv y bl =>
+      let x := match x with (x,x') => (f n x, x') end
+      with iv := map_invert (f n) iv
+      with y := f n y
+      with bl := Array.map (f n) bl in
+      make (Case info x iv y bl)
+  | Proj p r c =>
+      let c := f n c in
+      make (Proj p r c)
+  | Fix structs which tl bl =>
+      let (n,tl_l) := Ltac2.List.fold_right (fun b (n, l) => 
+        let (b', n') := lift n b in 
+        (n', List.cons b' l)) (Array.to_list tl) (n, []) in 
+      let tl := Array.of_list tl_l in
+      (* let n_bl := Array.fold_left lift n tl in *)
+      (* let bl := Array.map (f n_bl) bl in *)
+      make (Fix structs which tl (Array.map (f n) bl))
+  | CoFix which tl bl =>
+      let (n,tl_l) := Ltac2.List.fold_right (fun b (n, l) => 
+        let (b', n') := lift n b in 
+        (n', List.cons b' l)) (Array.to_list tl) (n, []) in 
+      let tl := Array.of_list tl_l in
+      make (CoFix which tl (Array.map (f n) bl))
+  | Array u t def ty =>
+      let ty := f n ty
+      with t := Array.map (f n) t
+      with def := f n def in
+      make (Array u t def ty)
+  end.
+
+(* Given a term, change the names of binders in that term to be fresh *)
+Ltac2 rec make_binders_distinct_aux (used : Fresh.Free.t) (c : constr) : constr :=
+  map_with_binders_alt (fun used b => 
+    match Binder.name b with
+    | None => (b, used)
+    | Some name => 
+      let newname := Fresh.fresh used name in 
+      let newused := Fresh.Free.union used (Fresh.Free.of_ids [newname]) in
+      (Binder.unsafe_make (Some newname) 
+        (Binder.relevance b) (Binder.type b),
+       newused)
+    end) (fun used c =>
+    make_binders_distinct_aux used c
+    ) used c.
+
+
+Ltac2 make_binders_distinct (c : constr) : constr :=
+  make_binders_distinct_aux
+    (Fresh.Free.of_ids []) c.
+
+(* Given a term, change the names of binders in that term to be anonymous *)
+Ltac2 rec make_binders_anon (c : constr) : constr :=
+  map_with_binders_alt (fun () b => 
+      (Binder.unsafe_make None (Binder.relevance b) (Binder.type b), ())
+    ) (fun () c =>
+    make_binders_anon c
+    ) () c.
+
+Ltac2 mk_evar (type : constr) : constr :=
+  (* TODO: investigate using Constr.pretype to avoid TC search *)
+  open_constr:(_ :> $type).
+
+Ltac2 unify_eq (c : constr) (d : constr) : bool :=
+  if Constr.equal c d then true else
+  if Int.equal (Control.numgoals()) 1 then
+    match Control.case (fun () => Std.unify c d) with
+    | Val _ => true
+    | Err _ => false
+    end
+  else false.
+
+
+Module Unsafe.
+
+Export Constr.Unsafe.
+
+Import PrintingExtra.Pp.
+
+
+Ltac2 rec decompose_lambda (f : constr) : binder * constr :=
+  match kind f with
+  | Lambda b c => (b, c)
+  | Cast c _ _ => decompose_lambda c
+  | _ => 
+    match kind (Std.eval_red f) with 
+    | Lambda b c => (b, c)
+    | _ => Control.throw (Invalid_argument (Some (str "decompose_lambda:" ++
+      spc() ++ str "constr" ++ spc() ++ Message.of_constr f ++ spc() ++
+      str "cannot be reduced to a bare lambda (by red)")))
+    end
+  end.
+
+Ltac2 rec decompose_prod (f : constr) : binder * constr :=
+  match kind f with
+  | Prod b c => (b, c)
+  | Cast c _ _ => decompose_prod c
+  | _ => 
+    match kind (Std.eval_red f) with 
+    | Lambda b c => (b, c)
+    | _ => Control.throw (Invalid_argument (Some (str "decompose_prod:" ++
+      spc() ++ str "constr" ++ spc() ++ Message.of_constr f ++ spc() ++
+      str "cannot be reduced to a bare prod (by red)")))
+    end
+  end.
+
+Ltac2 is_Rel_data (c : constr) : int option :=
+  match kind c with 
+  | Rel i => Some i
+  | _ => None
+  end.
+
+Ltac2 is_Var_data (c : constr) : ident option :=
+  match kind c with 
+  | Var i => Some i
+  | _ => None
+  end.
+
+Ltac2 mk_Rel (i : int) : constr :=
+  make (Rel i).
+
+(* Applies a funciton [f : constr -> constr] to [lem], where
+  [c] is [fun x y .. => lem x y ..] (i.e., strips off any lambda
+  binders and applies f to the inner function) *)
+Ltac2 rec map_lambda (f : constr -> constr) (c : constr) : constr :=
+  match Constr.Unsafe.kind c with 
+  | Constr.Unsafe.Lambda b body => 
+    let name := Option.default (Fresh.fresh (Fresh.Free.of_goal ()) ident:(x)) 
+      (Binder.name b) in 
+    Constr.in_context name (Binder.type b) (fun () => 
+    let c' := Constr.Unsafe.substnl [Control.hyp name] 0 body in 
+    let res := map_lambda f c' in 
+    Control.refine (fun _ => res))
+  | _ => f c
+  end.
+
+End Unsafe.
